Further work on the 3 Water Tanks case studies and algebraic loops.

Isabelle/INTO-CPS/INTO_SysML_3WTs_Pilot.thy
@@ -374,7 +374,7 @@ where
       ''wout'', ''win'', ''wlout'', ''vi1'', ''t3in'', ''t3wlout'', ''t3out'', ''vi2'',   
       ''din'', ''din'', ''wlin'', ''vo'',
       ''C_iout_t1in'', ''C_t1out_pin'', ''C_pout_t2in2'', ''C_t2out_wout'',
-      ''C_wout_win'', ''C_win_t3in'', ''C_t3lout_wlout'', ''C_t3out_din'',
+      ''C_wout_win'', ''C_win_t3in'', ''C_t3wlout_wlout'', ''C_t3out_din'',
       ''C_wlout_wlin'', ''C_vo_vi1'', ''C_vi1_vi2'',
       ''PrInflow_wout'', ''PrTankIO_win'', ''PrTankIO_wout'', ''PrPipe_win'',
       ''PrPipe_wout'', ''PrWaterTanks1_wout'', ''PrWaterTanks2_win'', 
@@ -385,7 +385,7 @@ where
     EsG = [''ECD_WTSys'', ''ECD_I'', ''ECD_P'', ''ECD_T1'', ''ECD_T2'', 
       ''ECD_T3'', ''ECD_C'', ''ECD_D'', ''ECD_WT1'', ''ECD_WT2'', 
       ''ECD_C_iout_t1in'', ''ECD_C_t1out_pin'', ''ECD_C_pout_t2in2'', ''ECD_C_t2out_wout'',
-      ''ECD_C_wout_win'', ''ECD_C_win_t3in'', ''ECD_C_t3lout_wlout'', ''ECD_C_t3out_din'',
+      ''ECD_C_wout_win'', ''ECD_C_win_t3in'', ''ECD_C_t3wlout_wlout'', ''ECD_C_t3out_din'',
       ''ECD_C_wlout_wlin'', ''ECD_C_vo_vi1'', ''ECD_C_vi1_vi2'',
       ''E_WTSys_WT1'', ''E_WTSys_WT2'', ''E_WTSys_C'',
       ''E_WT1_I'', ''E_WT1_P'', ''E_WT1_T1'', ''E_WT1_T2'', 
@@ -397,11 +397,11 @@ where
       ''E_WT2_wlout'', ''E_WT2_vi1'',
       ''E_C_iout_t1in_src'', ''E_C_iout_t1in_tgt'', 
       ''E_C_t1out_pin_src'', ''E_C_t1out_pin_tgt'', 
-      ''E_C_pout_t2in2_src'', ''E_C_pout_t2in2_tgt'',
+      ''E_C_pout_t2in_src'', ''E_C_pout_t2in_tgt'',
       ''E_C_t2out_wout_src'', ''E_C_t2out_wout_tgt'',
       ''E_C_wout_win_src'', ''E_C_wout_win_tgt'', 
       ''E_C_win_t3in_src'', ''E_C_win_t3in_tgt'', 
-      ''E_C_t3lout_wlout_src'', ''E_C_t3lout_wlout_tgt'', 
+      ''E_C_t3wlout_wlout_src'', ''E_C_t3wlout_wlout_tgt'', 
       ''E_C_t3out_din_src'', ''E_C_t3out_din_tgt'',
       ''E_C_wlout_wlin_src'', ''E_C_wlout_wlin_tgt'', 
       ''E_C_vo_vi1_src'', ''E_C_vo_vi1_tgt'', 
@@ -427,7 +427,7 @@ where
       (''ECD_C_iout_t1in'', ''CD_3WTs''), (''ECD_C_t1out_pin'', ''CD_3WTs''), 
       (''ECD_C_pout_t2in2'', ''CD_3WTs''), (''ECD_C_t2out_wout'', ''CD_3WTs''),
       (''ECD_C_wout_win'', ''CD_3WTs''), (''ECD_C_win_t3in'', ''CD_3WTs''),
-      (''ECD_C_t3lout_wlout'', ''CD_3WTs''), (''ECD_C_t3out_din'', ''CD_3WTs''),
+      (''ECD_C_t3wlout_wlout'', ''CD_3WTs''), (''ECD_C_t3out_din'', ''CD_3WTs''),
       (''ECD_C_wlout_wlin'', ''CD_3WTs''), (''ECD_C_vo_vi1'', ''CD_3WTs''), 
       (''ECD_C_vi1_vi2'', ''CD_3WTs''),
       (''E_WTSys_WT1'', ''WTSys''), (''E_WTSys_WT2'', ''WTSys''), 
@@ -446,16 +446,16 @@ where
       (''E_C_iout_t1in_tgt'', ''C_iout_t1in''),
       (''E_C_t1out_pin_src'', ''C_t1out_pin''), 
       (''E_C_t1out_pin_tgt'', ''C_t1out_pin''),
-      (''E_C_pout_t2in2_src'', ''C_pout_t2in2''), 
-      (''E_C_pout_t2in2_tgt'', ''C_pout_t2in2''),
+      (''E_C_pout_t2in_src'', ''C_pout_t2in2''), 
+      (''E_C_pout_t2in_tgt'', ''C_pout_t2in2''),
       (''E_C_t2out_wout_src'', ''C_t2out_wout''), 
       (''E_C_t2out_wout_tgt'', ''C_t2out_wout''),
       (''E_C_wout_win_src'', ''C_wout_win''), 
       (''E_C_wout_win_tgt'', ''C_wout_win''), 
       (''E_C_win_t3in_src'', ''C_win_t3in''),
       (''E_C_win_t3in_tgt'', ''C_win_t3in''),
-      (''E_C_t3lout_wlout_src'', ''C_t3lout_wlout''), 
-      (''E_C_t3lout_wlout_tgt'', ''C_t3lout_wlout''),
+      (''E_C_t3wlout_wlout_src'', ''C_t3wlout_wlout''), 
+      (''E_C_t3wlout_wlout_tgt'', ''C_t3wlout_wlout''),
       (''E_C_t3out_din_src'', ''C_t3out_din''),
       (''E_C_t3out_din_tgt'', ''C_t3out_din''),
       (''E_C_wlout_wlin_src'', ''C_wlout_wlin''),
@@ -504,7 +504,7 @@ where
       (''ECD_C_pout_t2in2'', ''C_pout_t2in2''), 
       (''ECD_C_t2out_wout'', ''C_t2out_wout''),
       (''ECD_C_wout_win'', ''C_wout_win''), (''ECD_C_win_t3in'', ''C_win_t3in''),
-      (''ECD_C_t3lout_wlout'', ''C_t3lout_wlout''), (''ECD_C_t3out_din'', ''C_t3out_din''),
+      (''ECD_C_t3wlout_wlout'', ''C_t3wlout_wlout''), (''ECD_C_t3out_din'', ''C_t3out_din''),
       (''ECD_C_wlout_wlin'', ''C_wlout_wlin''), (''ECD_C_vo_vi1'', ''C_vo_vi1''), 
       (''ECD_C_vi1_vi2'', ''C_vi1_vi2''),
       (''E_WTSys_WT1'', ''WT1''), (''E_WTSys_WT2'', ''WT2''), 
@@ -523,16 +523,16 @@ where
       (''E_C_iout_t1in_tgt'', ''t1in''),
       (''E_C_t1out_pin_src'', ''t1out''), 
       (''E_C_t1out_pin_tgt'', ''pin''),
-      (''E_C_pout_t2in2_src'', ''pout''), 
-      (''E_C_pout_t2in2_tgt'', ''t2in2''),
+      (''E_C_pout_t2in_src'', ''pout''), 
+      (''E_C_pout_t2in_tgt'', ''t2in''),
       (''E_C_t2out_wout_src'', ''t2out''), 
       (''E_C_t2out_wout_tgt'', ''wout''),
       (''E_C_wout_win_src'', ''wout''), 
       (''E_C_wout_win_tgt'', ''win''), 
       (''E_C_win_t3in_src'', ''win''),
       (''E_C_win_t3in_tgt'', ''t3in''),
-      (''E_C_t3lout_wlout_src'', ''t3lout''), 
-      (''E_C_t3lout_wlout_tgt'', ''wlout''),
+      (''E_C_t3wlout_wlout_src'', ''t3wlout''), 
+      (''E_C_t3wlout_wlout_tgt'', ''wlout''),
       (''E_C_t3out_din_src'', ''t3out''),
       (''E_C_t3out_din_tgt'', ''din''),
       (''E_C_wlout_wlin_src'', ''wlout''),
@@ -589,7 +589,7 @@ where
     (''din'', nnrml), (''din'', nnrml), (''wlin'', nnrml), (''vo'', nnrml),
     (''C_iout_t1in'', nnrml), (''C_t1out_pin'', nnrml), (''C_pout_t2in2'', nnrml),
     (''C_t2out_wout'', nnrml), (''C_wout_win'', nnrml), (''C_win_t3in'', nnrml), 
-    (''C_t3lout_wlout'', nnrml), (''C_t3out_din'', nnrml),
+    (''C_t3wlout_wlout'', nnrml), (''C_t3out_din'', nnrml),
     (''C_wlout_wlin'', nnrml), (''C_vo_vi1'', nnrml), (''C_vi1_vi2'', nnrml),
     (''PrInflow_wout'', nprxy), (''PrTankIO_win'', nprxy), (''PrTankIO_wout'', nprxy), 
     (''PrPipe_win'', nprxy), (''PrPipe_wout'', nprxy), (''PrWaterTanks1_wout'', nprxy), 
@@ -609,7 +609,7 @@ where
       (''ECD_C_pout_t2in2'', elnk), 
       (''ECD_C_t2out_wout'', elnk),
       (''ECD_C_wout_win'', elnk), (''ECD_C_win_t3in'', elnk),
-      (''ECD_C_t3lout_wlout'', elnk), (''ECD_C_t3out_din'', elnk),
+      (''ECD_C_t3wlout_wlout'', elnk), (''ECD_C_t3out_din'', elnk),
       (''ECD_C_wlout_wlin'', elnk), (''ECD_C_vo_vi1'', elnk), 
       (''ECD_C_vi1_vi2'', elnk),
       (''E_WTSys_WT1'', elnk), (''E_WTSys_WT2'', elnk), 
@@ -628,16 +628,16 @@ where
       (''E_C_iout_t1in_tgt'', elnk),
       (''E_C_t1out_pin_src'', elnk), 
       (''E_C_t1out_pin_tgt'', elnk),
-      (''E_C_pout_t2in2_src'', elnk), 
-      (''E_C_pout_t2in2_tgt'', elnk),
+      (''E_C_pout_t2in_src'', elnk), 
+      (''E_C_pout_t2in_tgt'', elnk),
       (''E_C_t2out_wout_src'', elnk), 
       (''E_C_t2out_wout_tgt'', elnk),
       (''E_C_wout_win_src'', elnk), 
       (''E_C_wout_win_tgt'', elnk), 
       (''E_C_win_t3in_src'', elnk),
       (''E_C_win_t3in_tgt'', elnk),
-      (''E_C_t3lout_wlout_src'', elnk), 
-      (''E_C_t3lout_wlout_tgt'', elnk),
+      (''E_C_t3wlout_wlout_src'', elnk), 
+      (''E_C_t3wlout_wlout_tgt'', elnk),
       (''E_C_t3out_din_src'', elnk),
       (''E_C_t3out_din_tgt'', elnk),
       (''E_C_wlout_wlin_src'', elnk),
@@ -691,7 +691,7 @@ where
 
 value "consInh SG_CD_3WTsP"
 
-lemma wf_SG_CD_3WTs: "is_wf_sg (toSGr SG_CD_3WTsP)"
+lemma wf_SG_CD_3WTsP: "is_wf_sg (toSGr SG_CD_3WTsP)"
   proof -
     have h_wf_g: "is_wf_g (toSGr SG_CD_3WTsP)"
     proof (simp add: is_wf_g_def, rule conjI)
@@ -708,21 +708,7 @@ lemma wf_SG_CD_3WTs: "is_wf_sg (toSGr SG_CD_3WTsP)"
     next
       show "ftotal_on (tgt (toSGr SG_CD_3WTsP)) (Es (toSGr SG_CD_3WTsP)) (Ns (toSGr SG_CD_3WTsP))"
       by (simp add: ftotal_on_def, rule conjI, simp add: SG_CD_3WTsP_def toSGr_def)
-        (rule subsetI, simp add: SG_CD_3WTsP_def toSGr_def, erule disjE, simp, 
-          erule disjE, simp, erule disjE, simp, erule disjE, simp, erule disjE, simp,
-          erule disjE, simp, erule disjE, simp, erule disjE, simp,
-          erule disjE, simp, erule disjE, simp, erule disjE, simp, erule disjE, simp,
-          erule disjE, simp, erule disjE, simp, erule disjE, simp, erule disjE, simp,
-          erule disjE, simp, erule disjE, simp, erule disjE, simp, erule disjE, simp,
-          erule disjE, simp, erule disjE, simp, erule disjE, simp, erule disjE, simp,
-          erule disjE, simp, erule disjE, simp, erule disjE, simp, erule disjE, simp,
-          erule disjE, simp, erule disjE, simp, erule disjE, simp, erule disjE, simp,
-          erule disjE, simp, erule disjE, simp, erule disjE, simp, erule disjE, simp,
-          erule disjE, simp, erule disjE, simp, erule disjE, simp, erule disjE, simp,
-          erule disjE, simp, erule disjE, simp, erule disjE, simp, erule disjE, simp,
-          erule disjE, simp, erule disjE, simp, erule disjE, simp, erule disjE, simp,
-          erule disjE, simp, erule disjE, simp, erule disjE, simp, erule disjE, simp,
-          erule disjE, simp, erule disjE, simp, erule disjE, simp, erule disjE, simp)
+        (rule subsetI, auto simp add: SG_CD_3WTsP_def toSGr_def)
     qed      
     show ?thesis
     proof (simp add: is_wf_sg_def, rule conjI)
@@ -770,164 +756,595 @@ lemma wf_SG_CD_3WTs: "is_wf_sg (toSGr SG_CD_3WTsP)"
 definition F_CD_3WTsP :: "Fr_ls"
 where
    "F_CD_3WTsP \<equiv> \<lparr>sg_ls = SG_CD_3WTsP, 
-    tr_ls = [(''ERPrWaterTank'', ''WaterTank''), (''ERPrValve'', ''Valve''), 
-    (''ERPrTanksControl1'', ''TanksControl1''), (''ERPrTanksControl2'', ''TanksControl2''),
-    (''ERPrController'', ''Controller''),
-    (''ERPrValve_v2'', ''Valve_v2''), (''ERPrValve_w'', ''Valve_w''), 
-    (''ERPrWaterTank_win'', ''WaterTank_win''),
-    (''ERPrWaterTank_wout'', ''WaterTank_wout''), 
-    (''ERPrController_v1'', ''Controller_v1'')]\<rparr>"
+    tr_ls = [(''ERPrTankIO'', ''TankIO''), (''ERPrTankIOV'', ''TankIOV''), 
+      (''ERPrInflow'', ''Inflow''), (''ERPrPipe'', ''Pipe''),
+      (''ERPrDrain'', ''Drain''),
+      (''ERPrWaterTanks1'', ''WaterTanks1''), (''ERPrWaterTanks2'', ''WaterTanks2''), 
+      (''ERPrController'', ''Controller''),
+      (''ERPrInflow_wout'', ''Inflow_wout''), 
+      (''ERPrTankIO_win'', ''TankIO_win''), 
+      (''ERPrTankIO_wout'', ''TankIO_wout''),
+      (''ERPrPipe_win'', ''Pipe_win''),
+      (''ERPrPipe_wout'', ''Pipe_wout''),
+      (''ERPrWaterTanks1_wout'', ''WaterTanks1_wout''),
+      (''ERPrWaterTanks2_win'', ''WaterTanks2_win''),
+      (''ERPrWaterTanks2_wlout'', ''WaterTanks2_wlout''),
+      (''ERPrWaterTanks2_vi'', ''WaterTanks2_vi''),
+      (''ERPrController_wlin'', ''Controller_wlin''),
+      (''ERPrController_vo'', ''Controller_vo''),
+      (''ERPrDrain_win'', ''Drain_win''),
+      (''ERPrTankIOV_win'', ''TankIOV_win''),
+      (''ERPrTankIOV_wout'', ''TankIOV_wout''),
+      (''ERPrTankIOV_wlout'', ''TankIOV_wlout''),
+      (''ERPrTankIOV_vi'', ''TankIOV_vi'')]\<rparr>"
 
-value "consRefs F_CD_3WTs"
+value "consRefs F_CD_3WTsP"
 
-value "consUFs [F_ASD_3WTs, F_CD_3WTs]"
+value "consUFs [F_ASD_3WTsP, F_CD_3WTsP]"
 
 (* Well-formedness proof obligation of fragments"*)
-lemma wf_F_CD_3WTs: "is_wf_fr (toFr F_CD_3WTs)"
+lemma wf_F_CD_3WTs: "is_wf_fr (toFr F_CD_3WTsP)"
   proof -
-    let ?refs_F_CD_3WTs = "{(''PrWaterTank'', ''WaterTank''), 
-      (''PrValve'', ''Valve''),
-      (''PrTanksControl1'', ''TanksControl1''), 
-      (''PrTanksControl2'', ''TanksControl2''),
-      (''PrController'', ''Controller''), 
-      (''PrValve_v2'', ''Valve_v2''),
-      (''PrValve_w'', ''Valve_w''), 
-      (''PrWaterTank_win'', ''WaterTank_win''),
-      (''PrWaterTank_wout'', ''WaterTank_wout''), 
-      (''PrController_v1'', ''Controller_v1'')}"
-    have h_EsRP: "EsRP (sg (toFr F_CD_3WTs)) = {''ERPrWaterTank'', ''ERPrValve'',
-          ''ERPrTanksControl1'', ''ERPrTanksControl2'',
-          ''ERPrController'', ''ERPrValve_v2'',
-          ''ERPrValve_w'', ''ERPrWaterTank_win'', 
-          ''ERPrWaterTank_wout'', ''ERPrController_v1''}"
+    let ?refs_F_CD_3WTsP = "{(''PrTankIO'', ''TankIO''), 
+      (''PrTankIOV'', ''TankIOV''), (''PrInflow'', ''Inflow''),
+      (''PrPipe'', ''Pipe''), (''PrDrain'', ''Drain''), 
+      (''PrWaterTanks1'', ''WaterTanks1''),
+      (''PrWaterTanks2'', ''WaterTanks2''), 
+      (''PrController'', ''Controller''),
+      (''PrInflow_wout'', ''Inflow_wout''), 
+      (''PrTankIO_win'', ''TankIO_win''),
+      (''PrTankIO_wout'', ''TankIO_wout''), 
+      (''PrPipe_win'', ''Pipe_win''),
+      (''PrPipe_wout'', ''Pipe_wout''), 
+      (''PrWaterTanks1_wout'', ''WaterTanks1_wout''),
+      (''PrWaterTanks2_win'', ''WaterTanks2_win''), 
+      (''PrWaterTanks2_wlout'', ''WaterTanks2_wlout''),
+      (''PrWaterTanks2_vi'', ''WaterTanks2_vi''), 
+      (''PrController_wlin'', ''Controller_wlin''),
+      (''PrController_vo'', ''Controller_vo''), 
+      (''PrDrain_win'', ''Drain_win''),
+      (''PrTankIOV_win'', ''TankIOV_win''), (''PrTankIOV_wout'', ''TankIOV_wout''),
+      (''PrTankIOV_wlout'', ''TankIOV_wlout''), (''PrTankIOV_vi'', ''TankIOV_vi'')}"
+    have h_EsRP: "EsRP (sg (toFr F_CD_3WTsP)) = {''ERPrTankIO'', ''ERPrTankIOV'', 
+      ''ERPrInflow'', ''ERPrPipe'', ''ERPrDrain'', ''ERPrWaterTanks1'', 
+      ''ERPrWaterTanks2'', ''ERPrController'', ''ERPrInflow_wout'', 
+      ''ERPrTankIO_win'', ''ERPrTankIO_wout'',
+      ''ERPrPipe_win'', ''ERPrPipe_wout'',
+      ''ERPrWaterTanks1_wout'', ''ERPrWaterTanks2_win'',
+      ''ERPrWaterTanks2_wlout'', ''ERPrWaterTanks2_vi'',
+      ''ERPrController_wlin'', ''ERPrController_vo'',
+      ''ERPrDrain_win'', ''ERPrTankIOV_win'',
+      ''ERPrTankIOV_wout'', ''ERPrTankIOV_wlout'', ''ERPrTankIOV_vi''}"
       by (rule equalityI, rule subsetI, simp_all add: EsRP_def EsR_def EsTy_def NsP_def NsTy_def 
-        toFr_def F_CD_3WTs_def toSGr_def SG_CD_3WTs_def split: if_splits)
-    have h_ftotal_tr: "ftotal_on (tr (toFr F_CD_3WTs)) (EsRP (sg (toFr F_CD_3WTs))) V_A"
-      using Ns_SG_ASD_3WTs
-      by (simp add: h_EsRP)(simp add: F_CD_3WTs_def SG_CD_3WTs_def toSGr_def toFr_def  
-          ftotal_on_def SG_ASD_3WTs_def) 
-    from wf_SG_CD_3WTs have hb: "is_wf_sg (sg (toFr F_CD_3WTs))"
-      by (simp add: toFr_def F_CD_3WTs_def)
-    have refs_F_CD_3WTs: "refs (toFr F_CD_3WTs) = ?refs_F_CD_3WTs"
+        toFr_def F_CD_3WTsP_def toSGr_def SG_CD_3WTsP_def split: if_splits)
+    have h_ftotal_tr: "ftotal_on (tr (toFr F_CD_3WTsP)) (EsRP (sg (toFr F_CD_3WTsP))) V_A"
+      using Ns_SG_ASD_3WTsP
+      by (simp add: h_EsRP)(simp add: F_CD_3WTsP_def SG_CD_3WTsP_def toSGr_def toFr_def  
+          ftotal_on_def SG_ASD_3WTsP_def) 
+    from wf_SG_CD_3WTsP have hb: "is_wf_sg (sg (toFr F_CD_3WTsP))"
+      by (simp add: toFr_def F_CD_3WTsP_def)
+    have refs_F_CD_3WTsP: "refs (toFr F_CD_3WTsP) = ?refs_F_CD_3WTsP"
       using h_ftotal_tr hb by (simp add: refs_eq_consRefs, eval)
-    have h_NsP: "NsP (sg (toFr F_CD_3WTs)) = {''PrWaterTank'', 
-      ''PrValve'', ''PrTanksControl1'', ''PrTanksControl2'', 
-      ''PrController'', ''PrValve_v2'', ''PrValve_w'', ''PrWaterTank_win'', 
-      ''PrWaterTank_wout'', ''PrController_v1''}"
-      by (rule equalityI, rule subsetI, simp_all add: F_CD_3WTs_def NsP_def NsTy_def 
-        toFr_def SG_CD_3WTs_def toSGr_def vimage_def split: if_splits)
+    have h_NsP: "NsP (sg (toFr F_CD_3WTsP)) = 
+      {''PrTankIO'', ''PrTankIOV'', ''PrInflow'',
+      ''PrPipe'', ''PrDrain'', ''PrWaterTanks1'',
+      ''PrWaterTanks2'', ''PrController'',
+      ''PrInflow_wout'', ''PrTankIO_win'',
+      ''PrTankIO_wout'', ''PrPipe_win'', ''PrPipe_wout'', 
+      ''PrWaterTanks1_wout'', ''PrWaterTanks2_win'', 
+      ''PrWaterTanks2_wlout'', ''PrWaterTanks2_vi'', 
+      ''PrController_wlin'', ''PrController_vo'', 
+      ''PrDrain_win'', ''PrTankIOV_win'', ''PrTankIOV_wout'',
+      ''PrTankIOV_wlout'', ''PrTankIOV_vi''}"
+      by (rule equalityI, rule subsetI, simp_all add: F_CD_3WTsP_def NsP_def NsTy_def 
+        toFr_def SG_CD_3WTsP_def toSGr_def vimage_def split: if_splits)
     show ?thesis
     proof (simp add: is_wf_fr_def)
       apply_end(rule conjI)
-      show "is_wf_sg (sg (toFr F_CD_3WTs))"  
-        by (simp add: wf_SG_CD_3WTs toFr_def F_CD_3WTs_def)
+      show "is_wf_sg (sg (toFr F_CD_3WTsP))"  
+        by (simp add: wf_SG_CD_3WTsP toFr_def F_CD_3WTsP_def)
     next
       apply_end(rule conjI) 
-      show "ftotal_on (tr (toFr F_CD_3WTs)) (EsRP (sg (toFr F_CD_3WTs))) V_A"
+      show "ftotal_on (tr (toFr F_CD_3WTsP)) (EsRP (sg (toFr F_CD_3WTsP))) V_A"
         by (simp add: h_ftotal_tr)
     next
       apply_end(rule conjI)  
-      show "inj_on (src (sg (toFr F_CD_3WTs))) (EsRP (sg (toFr F_CD_3WTs)))"
+      show "inj_on (src (sg (toFr F_CD_3WTsP))) (EsRP (sg (toFr F_CD_3WTsP)))"
       proof (simp add: inj_on_def, clarify)
         fix x y
-        assume "x \<in> EsRP (sg (toFr F_CD_3WTs))"
-          and "y \<in> EsRP (sg (toFr F_CD_3WTs))"
-          and "src (sg (toFr F_CD_3WTs)) x = src (sg (toFr F_CD_3WTs)) y"
-        then show "x = y"
-        by (simp add: h_EsRP) (simp add: F_CD_3WTs_def  
-          SG_CD_3WTs_def toFr_def toSGr_def split: if_splits) 
-      qed
-    next
-      apply_end(rule conjI)  
-      show "ran (src (sg (toFr F_CD_3WTs)) |` EsRP (sg (toFr F_CD_3WTs))) = NsP (sg (toFr F_CD_3WTs))"
-      by (simp add: h_EsRP h_NsP)(rule equalityI, simp_all add: F_CD_3WTs_def SG_CD_3WTs_def  
-        toFr_def toSGr_def)
-    next
-      apply_end(rule conjI)
-      show "\<forall>v. v \<in> NsP (sg (toFr F_CD_3WTs)) \<longrightarrow> nonPRefsOf (toFr F_CD_3WTs) v \<noteq> {}"
-      proof (rule allI, rule impI)
-        fix v
-        assume h1: "v \<in> NsP (sg (toFr F_CD_3WTs))"
-        then show "nonPRefsOf (toFr F_CD_3WTs) v \<noteq> {}"
-        proof (case_tac  "v = ''PrWaterTank''")
-          assume "v = ''PrWaterTank''"
-          then show "nonPRefsOf (toFr F_CD_3WTs) v \<noteq> {}"
-            by (simp add: h_NsP nonPRefsOf_def refsOf_def refs_F_CD_3WTs trancl_in)
-        next  
-          assume h2: "v \<noteq> ''PrWaterTank''"
-          then show "nonPRefsOf (toFr F_CD_3WTs) v \<noteq> {}"
-          proof (case_tac  "v = ''PrValve''")
-            assume "v = ''PrValve''"
-            then show "nonPRefsOf (toFr F_CD_3WTs) v \<noteq> {}"
-              by (simp add: h_NsP nonPRefsOf_def refsOf_def refs_F_CD_3WTs trancl_in)
+        assume h1: "x \<in> EsRP (sg (toFr F_CD_3WTsP))"
+          and h2: "y \<in> EsRP (sg (toFr F_CD_3WTsP))"
+          and h3: "src (sg (toFr F_CD_3WTsP)) x = src (sg (toFr F_CD_3WTsP)) y"
+        show "x = y"
+        proof (case_tac  "y = ''ERPrTankIO''")
+          assume "y = ''ERPrTankIO''"
+          then show "x = y"
+          using h1 h2 h3 by (simp add: h_EsRP)(simp add: F_CD_3WTsP_def EsRP_def EsR_def EsTy_def
+            SG_CD_3WTsP_def toFr_def toSGr_def split: if_splits)
+        next
+          assume h4: "y \<noteq> ''ERPrTankIO''" 
+          then show "x = y"
+          proof (case_tac  "y = ''ERPrTankIOV''")
+            assume "y = ''ERPrTankIOV''"
+            then show "x = y"
+            using h1 h2 h3 by (simp add: h_EsRP)(simp add: F_CD_3WTsP_def EsRP_def EsR_def EsTy_def
+              SG_CD_3WTsP_def toFr_def toSGr_def split: if_splits)
           next
-            assume h3: "v \<noteq> ''PrValve''"
-            then show "nonPRefsOf (toFr F_CD_3WTs) v \<noteq> {}"
-            proof (case_tac  "v = ''PrTanksControl1''")
-              assume "v = ''PrTanksControl1''"
-              then show "nonPRefsOf (toFr F_CD_3WTs) v \<noteq> {}"
-                by (simp add: h_NsP nonPRefsOf_def refsOf_def refs_F_CD_3WTs trancl_in)
+            assume h5: "y \<noteq> ''ERPrTankIOV''"
+            then show "x = y"
+            proof (case_tac  "y = ''ERPrInflow''")
+              assume "y = ''ERPrInflow''"
+              then show "x = y"
+              using h1 h2 h3 by (simp add: h_EsRP)(simp add: F_CD_3WTsP_def EsRP_def EsR_def EsTy_def
+                SG_CD_3WTsP_def toFr_def toSGr_def split: if_splits)
             next
-              assume h4: "v \<noteq> ''PrTanksControl1''"
-              then show "nonPRefsOf (toFr F_CD_3WTs) v \<noteq> {}"
-              proof (case_tac  "v = ''PrTanksControl2''")
-                assume "v = ''PrTanksControl2''"
-                then show "nonPRefsOf (toFr F_CD_3WTs) v \<noteq> {}"
-                  by (simp add: h_NsP nonPRefsOf_def refsOf_def refs_F_CD_3WTs trancl_in)
+              assume h6: "y \<noteq> ''ERPrInflow''"
+              then show "x = y"
+              proof (case_tac  "y = ''ERPrPipe''")
+                assume "y = ''ERPrPipe''"
+                then show "x = y"
+                using h1 h2 h3 by (simp add: h_EsRP)(simp add: F_CD_3WTsP_def EsRP_def EsR_def EsTy_def
+                  SG_CD_3WTsP_def toFr_def toSGr_def split: if_splits)
               next
-                assume h5: "v \<noteq> ''PrTanksControl2''"
-                then show "nonPRefsOf (toFr F_CD_3WTs) v \<noteq> {}"
-                proof (case_tac  "v = ''PrController''")
-                  assume "v = ''PrController''"
-                  then show "nonPRefsOf (toFr F_CD_3WTs) v \<noteq> {}"
-                    by (simp add: h_NsP nonPRefsOf_def refsOf_def refs_F_CD_3WTs trancl_in)
+                assume h7: "y \<noteq> ''ERPrPipe''"
+                then show "x = y"
+                proof (case_tac "y = ''ERPrDrain''")
+                  assume "y = ''ERPrDrain''"
+                  then show "x = y"
+                  using h1 h2 h3 by (simp add: h_EsRP)(simp add: F_CD_3WTsP_def EsRP_def EsR_def EsTy_def
+                    SG_CD_3WTsP_def toFr_def toSGr_def split: if_splits)
                 next
-                  assume h6: "v \<noteq> ''PrController''"
-                  then show "nonPRefsOf (toFr F_CD_3WTs) v \<noteq> {}"
-                  proof (case_tac "v = ''PrValve_v2''")
-                    assume "v = ''PrValve_v2''"
-                    then show "nonPRefsOf (toFr F_CD_3WTs) v \<noteq> {}"
-                      by (simp add: h_NsP nonPRefsOf_def refsOf_def refs_F_CD_3WTs trancl_in)
+                  assume h8: "y \<noteq> ''ERPrDrain''"
+                  then show "x = y"
+                  proof (case_tac "y = ''ERPrWaterTanks1''")
+                    assume "y = ''ERPrWaterTanks1''"
+                    then show "x = y"
+                    using h1 h2 h3 by (simp add: h_EsRP)
+                      (simp add: F_CD_3WTsP_def EsRP_def EsR_def EsTy_def
+                      SG_CD_3WTsP_def toFr_def toSGr_def split: if_splits)
                   next
-                    assume h7: "v \<noteq> ''PrValve_v2''"
-                    then show "nonPRefsOf (toFr F_CD_3WTs) v \<noteq> {}"
-                    proof (case_tac "v = ''PrValve_w''")
-                      assume "v = ''PrValve_w''"
-                      then show "nonPRefsOf (toFr F_CD_3WTs) v \<noteq> {}"
-                        by (simp add: h_NsP nonPRefsOf_def refsOf_def refs_F_CD_3WTs trancl_in)
+                    assume h9: "y \<noteq> ''ERPrWaterTanks1''"
+                    then show "x = y"
+                    proof (case_tac "y = ''ERPrWaterTanks2''")
+                      assume "y = ''ERPrWaterTanks2''"
+                      then show "x = y"
+                      using h1 h2 h3 by (simp add: h_EsRP)
+                        (simp add: F_CD_3WTsP_def EsRP_def EsR_def EsTy_def
+                        SG_CD_3WTsP_def toFr_def toSGr_def split: if_splits)
                     next
-                      assume h8: "v \<noteq> ''PrValve_w''"
-                      then show "nonPRefsOf (toFr F_CD_3WTs) v \<noteq> {}"
-                      proof (case_tac "v = ''PrWaterTank_win''")
-                        assume "v = ''PrWaterTank_win''"
-                        then show "nonPRefsOf (toFr F_CD_3WTs) v \<noteq> {}"
-                          by (simp add: h_NsP nonPRefsOf_def refsOf_def refs_F_CD_3WTs trancl_in)
+                      assume h10: "y \<noteq> ''ERPrWaterTanks2''"
+                      then show "x = y"
+                      proof (case_tac "y = ''ERPrController''")
+                        assume "y = ''ERPrController''"
+                        then show "x = y"
+                        using h1 h2 h3 by (simp add: h_EsRP)
+                          (simp add: F_CD_3WTsP_def EsRP_def EsR_def EsTy_def
+                            SG_CD_3WTsP_def toFr_def toSGr_def split: if_splits)
                       next
-                        assume h9: "v \<noteq> ''PrWaterTank_win''"
-                        then show "nonPRefsOf (toFr F_CD_3WTs) v \<noteq> {}"
-                        proof (case_tac "v = ''PrWaterTank_wout''")
-                          assume "v = ''PrWaterTank_wout''"
-                          then show "nonPRefsOf (toFr F_CD_3WTs) v \<noteq> {}"
-                            by (simp add: h_NsP nonPRefsOf_def refsOf_def refs_F_CD_3WTs trancl_in)
+                        assume h11: "y \<noteq> ''ERPrController''"
+                        then show "x = y"
+                        proof (case_tac "y = ''ERPrInflow_wout''")
+                          assume "y = ''ERPrInflow_wout''"
+                          then show "x = y"
+                          using h1 h2 h3 by (simp add: h_EsRP)
+                            (simp add: F_CD_3WTsP_def EsRP_def EsR_def EsTy_def
+                              SG_CD_3WTsP_def toFr_def toSGr_def split: if_splits)
                         next
-                          assume h10: "v \<noteq> ''PrWaterTank_wout''"
-                          then show "nonPRefsOf (toFr F_CD_3WTs) v \<noteq> {}"
-                          using h2 h3 h4 h5 h6 h7 h8 h9 
-                          proof (case_tac "v = ''PrController_v1''")
-                            assume "v = ''PrController_v1''"
-                            then show "nonPRefsOf (toFr F_CD_3WTs) v \<noteq> {}"
-                              by (simp add: h_NsP nonPRefsOf_def refsOf_def refs_F_CD_3WTs 
-                                trancl_in)
+                          assume h12: "y \<noteq> ''ERPrInflow_wout''"
+                          then show "x = y"
+                          proof (case_tac "y = ''ERPrTankIO_win''")
+                            assume "y = ''ERPrTankIO_win''"
+                            then show "x = y"
+                            using h1 h2 h3 by (simp add: h_EsRP)
+                              (simp add: F_CD_3WTsP_def EsRP_def EsR_def EsTy_def
+                              SG_CD_3WTsP_def toFr_def toSGr_def split: if_splits)
                           next
-                            assume "v \<noteq> ''PrController_v1''"
-                            show "nonPRefsOf (toFr F_CD_3WTs) v \<noteq> {}"
-                            using h1 h2 h3 h4 h5 h6 h7 h8 h9 h10 
-                              by (auto simp add: h_NsP nonPRefsOf_def refsOf_def refs_F_CD_3WTs image_def)
+                            assume h13: "y \<noteq> ''ERPrTankIO_win''"
+                            then show "x = y"
+                            proof (case_tac "y = ''ERPrTankIO_wout''")
+                              assume "y = ''ERPrTankIO_wout''"
+                              then show "x = y"
+                                using h1 h2 h3 by (simp add: h_EsRP)
+                                (simp add: F_CD_3WTsP_def EsRP_def EsR_def EsTy_def
+                                  SG_CD_3WTsP_def toFr_def toSGr_def split: if_splits)
+                            next
+                              assume h14: "y \<noteq> ''ERPrTankIO_wout''"
+                              then show "x = y"
+                              proof (case_tac "y = ''ERPrPipe_win''")
+                                assume "y = ''ERPrPipe_win''"
+                                then show "x = y"
+                                using h1 h2 h3 by (simp add: h_EsRP)
+                                  (simp add: F_CD_3WTsP_def EsRP_def EsR_def EsTy_def
+                                    SG_CD_3WTsP_def toFr_def toSGr_def split: if_splits)
+                              next
+                                assume h15: "y \<noteq> ''ERPrPipe_win''"
+                                then show "x = y"
+                                proof (case_tac "y = ''ERPrPipe_wout''")
+                                  assume "y = ''ERPrPipe_wout''"
+                                  then show "x = y"
+                                  using h1 h2 h3 by (simp add: h_EsRP)
+                                    (simp add: F_CD_3WTsP_def EsRP_def EsR_def EsTy_def
+                                    SG_CD_3WTsP_def toFr_def toSGr_def split: if_splits)
+                                next
+                                  assume h16: "y \<noteq> ''ERPrPipe_wout''"
+                                  then show "x = y"
+                                  proof (case_tac "y = ''ERPrWaterTanks1_wout''")
+                                    assume "y = ''ERPrWaterTanks1_wout''"
+                                    then show "x = y"
+                                    using h1 h2 h3 by (simp add: h_EsRP)
+                                      (simp add: F_CD_3WTsP_def EsRP_def EsR_def EsTy_def
+                                        SG_CD_3WTsP_def toFr_def toSGr_def split: if_splits)
+                                  next
+                                    assume h17: "y \<noteq> ''ERPrWaterTanks1_wout''"
+                                    then show "x = y"
+                                    proof (case_tac "y = ''ERPrWaterTanks2_win''")
+                                      assume "y = ''ERPrWaterTanks2_win''"
+                                      then show "x = y"
+                                      using h1 h2 h3 by (simp add: h_EsRP)
+                                      (simp add: F_CD_3WTsP_def EsRP_def EsR_def EsTy_def
+                                        SG_CD_3WTsP_def toFr_def toSGr_def split: if_splits)
+                                    next
+                                      assume h18: "y \<noteq> ''ERPrWaterTanks2_win''"
+                                      then show "x = y"
+                                      proof (case_tac "y = ''ERPrWaterTanks2_wlout''")
+                                        assume "y = ''ERPrWaterTanks2_wlout''"
+                                        then show "x = y"
+                                        using h1 h2 h3 by (simp add: h_EsRP)
+                                        (simp add: F_CD_3WTsP_def EsRP_def EsR_def EsTy_def
+                                          SG_CD_3WTsP_def toFr_def toSGr_def split: if_splits)
+                                      next
+                                        assume h19: "y \<noteq> ''ERPrWaterTanks2_wlout''"
+                                        then show "x = y"
+                                        proof (case_tac "y=''ERPrWaterTanks2_vi''")
+                                          assume "y=''ERPrWaterTanks2_vi''"
+                                          then show "x = y"
+                                          using h1 h2 h3 by (simp add: h_EsRP)
+                                          (simp add: F_CD_3WTsP_def EsRP_def EsR_def EsTy_def
+                                            SG_CD_3WTsP_def toFr_def toSGr_def split: if_splits)
+                                        next
+                                          assume h20: "y \<noteq> ''ERPrWaterTanks2_vi''"
+                                          then show "x = y"
+                                          proof (case_tac "y=''ERPrController_wlin''")
+                                            assume "y=''ERPrController_wlin''"
+                                            then show "x = y"
+                                            using h1 h2 h3 by (simp add: h_EsRP)
+                                            (simp add: F_CD_3WTsP_def EsRP_def EsR_def EsTy_def
+                                            SG_CD_3WTsP_def toFr_def toSGr_def split: if_splits)
+                                          next
+                                            assume h21: "y\<noteq>''ERPrController_wlin''" 
+                                            then show "x = y"
+                                            proof (case_tac "y=''ERPrController_vo''")
+                                              assume "y = ''ERPrController_vo''"
+                                              then show "x = y"
+                                              using h1 h2 h3 by (simp add: h_EsRP)
+                                              (simp add: F_CD_3WTsP_def EsRP_def EsR_def EsTy_def
+                                                  SG_CD_3WTsP_def toFr_def toSGr_def split: if_splits)
+                                            next
+                                              assume h22: "y \<noteq> ''ERPrController_vo''"
+                                              then show "x = y"
+                                              proof (case_tac "y = ''ERPrDrain_win''")
+                                                assume "y = ''ERPrDrain_win''"
+                                                then show "x = y"
+                                                using h1 h2 h3 by (simp add: h_EsRP)
+                                                (simp add: F_CD_3WTsP_def EsRP_def EsR_def EsTy_def
+                                                  SG_CD_3WTsP_def toFr_def toSGr_def split: if_splits)
+                                              next
+                                                assume h23: "y \<noteq> ''ERPrDrain_win''"
+                                                then show "x = y"
+                                                proof (case_tac "y = ''ERPrTankIOV_win''")
+                                                  assume "y = ''ERPrTankIOV_win''"
+                                                  then show "x = y"
+                                                  using h1 h2 h3 by (simp add: h_EsRP)
+                                                  (simp add: F_CD_3WTsP_def EsRP_def EsR_def 
+                                                    EsTy_def
+                                                  SG_CD_3WTsP_def toFr_def toSGr_def split: if_splits)
+                                                next
+                                                  assume h24: "y \<noteq> ''ERPrTankIOV_win''"
+                                                  then show "x = y"
+                                                  proof (case_tac "y = ''ERPrTankIOV_wout''")
+                                                    assume "y = ''ERPrTankIOV_wout''"
+                                                    then show "x = y"
+                                                    using h1 h2 h3 by (simp add: h_EsRP)
+                                                    (simp add: F_CD_3WTsP_def EsRP_def EsR_def 
+                                                    EsTy_def
+                                                    SG_CD_3WTsP_def toFr_def toSGr_def split: if_splits)
+                                                  next
+                                                    assume h25: "y \<noteq> ''ERPrTankIOV_wout''"
+                                                    then show "x = y"
+                                                    proof (case_tac "y = ''ERPrTankIOV_wlout''")
+                                                      assume "y = ''ERPrTankIOV_wlout''"
+                                                      then show "x = y"
+                                                      using h1 h2 h3 by (simp add: h_EsRP)
+                                                      (simp add: F_CD_3WTsP_def EsRP_def EsR_def 
+                                                        EsTy_def
+                                                        SG_CD_3WTsP_def toFr_def 
+                                                        toSGr_def split: if_splits)
+                                                    next
+                                                      assume h26: "y \<noteq> ''ERPrTankIOV_wlout''"
+                                                      then show "x = y"
+                                                      proof (case_tac "y = ''ERPrTankIOV_vi''")
+                                                        assume "y = ''ERPrTankIOV_vi''"
+                                                        then show "x = y"
+                                                        using h1 h2 h3 by (simp add: h_EsRP)
+                                                        (simp add: F_CD_3WTsP_def EsRP_def EsR_def 
+                                                          EsTy_def SG_CD_3WTsP_def toFr_def 
+                                                          toSGr_def split: if_splits)
+                                                      next  
+                                                        assume "y \<noteq> ''ERPrTankIOV_vi''"
+                                                        then show "x = y"
+                                                        using h1 h2 h4 h5 h6 h7 h8 h9 h10 h11 h12
+                                                        h13 h14 h15 h16 h17 h18 h19 h20 h21 
+                                                        h22 h23 h24 h25 h26 
+                                                        by (simp add: h_EsRP)
+                                                      qed
+                                                    qed
+                                                  qed
+                                                qed
+                                              qed
+                                            qed
+                                          qed
+                                        qed
+                                      qed
+                                    qed
+                                  qed
+                                qed
+                              qed
+                            qed
                           qed
                         qed
                       qed
                     qed
-                  qed 
+                  qed
+                qed
+              qed
+            qed
+          qed
+        qed
+      qed
+    next
+      apply_end(rule conjI)  
+      show "ran (src (sg (toFr F_CD_3WTsP)) |` EsRP (sg (toFr F_CD_3WTsP))) = NsP (sg (toFr F_CD_3WTsP))"
+      by (simp add: h_EsRP h_NsP)(rule equalityI, simp_all add: F_CD_3WTsP_def SG_CD_3WTsP_def  
+        toFr_def toSGr_def)
+    next
+      apply_end(rule conjI)
+      show "\<forall>v. v \<in> NsP (sg (toFr F_CD_3WTsP)) \<longrightarrow> nonPRefsOf (toFr F_CD_3WTsP) v \<noteq> {}"
+      proof (rule allI, rule impI)
+        fix v
+        assume h1: "v \<in> NsP (sg (toFr F_CD_3WTsP))"
+        then show "nonPRefsOf (toFr F_CD_3WTsP) v \<noteq> {}"
+        proof (case_tac  "v = ''PrTankIO''")
+          assume "v = ''PrTankIO''"
+          then show "nonPRefsOf (toFr F_CD_3WTsP) v \<noteq> {}"
+            by (simp add: h_NsP nonPRefsOf_def refsOf_def refs_F_CD_3WTsP trancl_in)
+        next  
+          assume h2: "v \<noteq> ''PrTankIO''"
+          then show "nonPRefsOf (toFr F_CD_3WTsP) v \<noteq> {}"
+          proof (case_tac  "v = ''PrTankIOV''")
+            assume "v = ''PrTankIOV''"
+            then show "nonPRefsOf (toFr F_CD_3WTsP) v \<noteq> {}"
+              by (simp add: h_NsP nonPRefsOf_def refsOf_def refs_F_CD_3WTsP trancl_in)
+          next
+            assume h3: "v \<noteq> ''PrTankIOV''"
+            then show "nonPRefsOf (toFr F_CD_3WTsP) v \<noteq> {}"
+            proof (case_tac  "v = ''PrPipe''")
+              assume "v = ''PrPipe''"
+              then show "nonPRefsOf (toFr F_CD_3WTsP) v \<noteq> {}"
+                by (simp add: h_NsP nonPRefsOf_def refsOf_def refs_F_CD_3WTsP trancl_in)
+            next
+              assume h4: "v \<noteq> ''PrPipe''"
+              then show "nonPRefsOf (toFr F_CD_3WTsP) v \<noteq> {}"
+              proof (case_tac  "v = ''PrDrain''")
+                assume "v = ''PrDrain''"
+                then show "nonPRefsOf (toFr F_CD_3WTsP) v \<noteq> {}"
+                  by (simp add: h_NsP nonPRefsOf_def refsOf_def refs_F_CD_3WTsP trancl_in)
+              next
+                assume h5: "v \<noteq> ''PrDrain''"
+                then show "nonPRefsOf (toFr F_CD_3WTsP) v \<noteq> {}"
+                proof (case_tac  "v = ''PrWaterTanks1''")
+                  assume "v = ''PrWaterTanks1''"
+                  then show "nonPRefsOf (toFr F_CD_3WTsP) v \<noteq> {}"
+                    by (simp add: h_NsP nonPRefsOf_def refsOf_def refs_F_CD_3WTsP trancl_in)
+                next
+                  assume h6: "v \<noteq> ''PrWaterTanks1''"
+                  then show "nonPRefsOf (toFr F_CD_3WTsP) v \<noteq> {}"
+                  proof (case_tac "v = ''PrWaterTanks2''")
+                    assume "v = ''PrWaterTanks2''"
+                    then show "nonPRefsOf (toFr F_CD_3WTsP) v \<noteq> {}"
+                      by (simp add: h_NsP nonPRefsOf_def refsOf_def refs_F_CD_3WTsP trancl_in)
+                  next
+                    assume h7: "v \<noteq> ''PrWaterTanks2''"
+                    then show "nonPRefsOf (toFr F_CD_3WTsP) v \<noteq> {}"
+                    proof (case_tac "v = ''PrController_wlin''")
+                      assume "v = ''PrController_wlin''"
+                      then show "nonPRefsOf (toFr F_CD_3WTsP) v \<noteq> {}"
+                        by (simp add: h_NsP nonPRefsOf_def refsOf_def refs_F_CD_3WTsP trancl_in)
+                    next
+                      assume h8: "v \<noteq> ''PrController_wlin''"
+                      then show "nonPRefsOf (toFr F_CD_3WTsP) v \<noteq> {}"
+                      proof (case_tac "v = ''PrInflow_wout''")
+                        assume "v = ''PrInflow_wout''"
+                        then show "nonPRefsOf (toFr F_CD_3WTsP) v \<noteq> {}"
+                          by (simp add: h_NsP nonPRefsOf_def refsOf_def refs_F_CD_3WTsP trancl_in)
+                      next
+                        assume h9: "v \<noteq> ''PrInflow_wout''"
+                        then show "nonPRefsOf (toFr F_CD_3WTsP) v \<noteq> {}"
+                        proof (case_tac "v = ''PrTankIO_win''")
+                          assume "v = ''PrTankIO_win''"
+                          then show "nonPRefsOf (toFr F_CD_3WTsP) v \<noteq> {}"
+                            by (simp add: h_NsP nonPRefsOf_def refsOf_def refs_F_CD_3WTsP trancl_in)
+                        next
+                          assume h10: "v \<noteq> ''PrTankIO_win''"
+                          then show "nonPRefsOf (toFr F_CD_3WTsP) v \<noteq> {}"
+                          proof (case_tac "v = ''PrController_wlin''")
+                            assume "v = ''PrController_wlin''"
+                            then show "nonPRefsOf (toFr F_CD_3WTsP) v \<noteq> {}"
+                              by (simp add: h_NsP nonPRefsOf_def refsOf_def refs_F_CD_3WTsP 
+                                trancl_in)
+                          next
+                            assume h11: "v \<noteq> ''PrController_wlin''"
+                            then show "nonPRefsOf (toFr F_CD_3WTsP) v \<noteq> {}"
+                            proof (case_tac "v = ''PrController_vo''")
+                              assume "v = ''PrController_vo''"
+                              then show "nonPRefsOf (toFr F_CD_3WTsP) v \<noteq> {}"
+                              by (simp add: h_NsP nonPRefsOf_def refsOf_def refs_F_CD_3WTsP 
+                                trancl_in)
+                            next
+                              assume h12: "v \<noteq> ''PrController_vo''"
+                              then show "nonPRefsOf (toFr F_CD_3WTsP) v \<noteq> {}"
+                              proof (case_tac "v = ''PrDrain_win''")
+                                assume "v = ''PrDrain_win''"
+                                then show "nonPRefsOf (toFr F_CD_3WTsP) v \<noteq> {}"
+                                by (simp add: h_NsP nonPRefsOf_def refsOf_def refs_F_CD_3WTsP 
+                                  trancl_in)
+                              next
+                                assume h13: "v \<noteq> ''PrDrain_win''"
+                                then show "nonPRefsOf (toFr F_CD_3WTsP) v \<noteq> {}"
+                                proof (case_tac "v = ''PrTankIOV_win''")
+                                  assume "v = ''PrTankIOV_win''"
+                                  then show "nonPRefsOf (toFr F_CD_3WTsP) v \<noteq> {}"
+                                    by (simp add: h_NsP nonPRefsOf_def refsOf_def refs_F_CD_3WTsP 
+                                  trancl_in)
+                                next
+                                  assume h14: "v \<noteq> ''PrTankIOV_win''"
+                                  then show "nonPRefsOf (toFr F_CD_3WTsP) v \<noteq> {}"
+                                  proof (case_tac "v = ''PrTankIOV_wout''")
+                                    assume "v = ''PrTankIOV_wout''"
+                                    then show "nonPRefsOf (toFr F_CD_3WTsP) v \<noteq> {}"
+                                    by (simp add: h_NsP nonPRefsOf_def refsOf_def refs_F_CD_3WTsP 
+                                      trancl_in)
+                                  next
+                                    assume h15: "v \<noteq> ''PrTankIOV_wout''"
+                                    then show "nonPRefsOf (toFr F_CD_3WTsP) v \<noteq> {}"
+                                    proof (case_tac "v = ''PrTankIOV_wlout''")
+                                      assume "v = ''PrTankIOV_wlout''"
+                                      then show "nonPRefsOf (toFr F_CD_3WTsP) v \<noteq> {}"
+                                      by (simp add: h_NsP nonPRefsOf_def refsOf_def refs_F_CD_3WTsP 
+                                        trancl_in)
+                                    next
+                                      assume h16: "v \<noteq> ''PrTankIOV_wlout''"
+                                      then show "nonPRefsOf (toFr F_CD_3WTsP) v \<noteq> {}"
+                                      proof (case_tac "v = ''PrTankIOV_vi''")
+                                        assume "v = ''PrTankIOV_vi''"
+                                        then show "nonPRefsOf (toFr F_CD_3WTsP) v \<noteq> {}"
+                                        by (simp add: h_NsP nonPRefsOf_def refsOf_def refs_F_CD_3WTsP 
+                                        trancl_in)
+                                      next
+                                        assume "v \<noteq> ''PrTankIOV_vi''"
+                                        then show "nonPRefsOf (toFr F_CD_3WTsP) v \<noteq> {}"
+                                        proof (case_tac "v = ''PrInflow''")
+                                          assume "v = ''PrInflow''"
+                                          then show "nonPRefsOf (toFr F_CD_3WTsP) v \<noteq> {}"
+                                          by (simp add: h_NsP nonPRefsOf_def refsOf_def refs_F_CD_3WTsP 
+                                            trancl_in)
+                                        next
+                                          assume h17: "v \<noteq> ''PrInflow''"
+                                          then show "nonPRefsOf (toFr F_CD_3WTsP) v \<noteq> {}"
+                                          proof (case_tac "v = ''PrController''")
+                                            assume "v = ''PrController''"
+                                            then show "nonPRefsOf (toFr F_CD_3WTsP) v \<noteq> {}"
+                                            by (simp add: h_NsP nonPRefsOf_def refsOf_def refs_F_CD_3WTsP 
+                                              trancl_in)
+                                          next
+                                            assume h18: "v \<noteq>''PrController''"
+                                            then show "nonPRefsOf (toFr F_CD_3WTsP) v \<noteq> {}"
+                                            proof (case_tac "v = ''PrTankIO_wout''")
+                                              assume "v = ''PrTankIO_wout''"
+                                              then show "nonPRefsOf (toFr F_CD_3WTsP) v \<noteq> {}"
+                                              by (simp add: h_NsP nonPRefsOf_def refsOf_def refs_F_CD_3WTsP 
+                                                trancl_in)
+                                            next
+                                              assume h19: "v \<noteq> ''PrTankIO_wout''"
+                                              then show "nonPRefsOf (toFr F_CD_3WTsP) v \<noteq> {}"
+                                              proof (case_tac "v = ''PrPipe_win''")
+                                                assume "v = ''PrPipe_win''"
+                                                then show "nonPRefsOf (toFr F_CD_3WTsP) v \<noteq> {}"
+                                                by (simp add: h_NsP nonPRefsOf_def refsOf_def refs_F_CD_3WTsP 
+                                                  trancl_in)
+                                              next
+                                                assume h20: "v \<noteq> ''PrPipe_win''"
+                                                then show "nonPRefsOf (toFr F_CD_3WTsP) v \<noteq> {}"
+                                                proof (case_tac "v = ''PrPipe_wout''")
+                                                  assume "v = ''PrPipe_wout''"
+                                                  then show "nonPRefsOf (toFr F_CD_3WTsP) v \<noteq> {}"
+                                                  by (simp add: h_NsP nonPRefsOf_def refsOf_def refs_F_CD_3WTsP 
+                                                  trancl_in)
+                                                next
+                                                  assume h21: "v \<noteq> ''PrPipe_wout''"
+                                                  then show "nonPRefsOf (toFr F_CD_3WTsP) v \<noteq> {}"
+                                                  proof (case_tac "v = ''PrWaterTanks1_wout''")
+                                                    assume "v = ''PrWaterTanks1_wout''"
+                                                    then show "nonPRefsOf (toFr F_CD_3WTsP) v \<noteq> {}"
+                                                    by (simp add: h_NsP nonPRefsOf_def refsOf_def refs_F_CD_3WTsP 
+                                                      trancl_in)
+                                                  next
+                                                    assume h22: "v \<noteq> ''PrWaterTanks1_wout''"
+                                                    then show "nonPRefsOf (toFr F_CD_3WTsP) v \<noteq> {}"
+                                                    proof (case_tac "v = ''PrWaterTanks1_wout''")
+                                                      assume "v = ''PrWaterTanks1_wout''"
+                                                      then show "nonPRefsOf (toFr F_CD_3WTsP) v \<noteq> {}"
+                                                      by (simp add: h_NsP nonPRefsOf_def refsOf_def refs_F_CD_3WTsP 
+                                                      trancl_in)
+                                                    next
+                                                      assume h23: "v \<noteq> ''PrWaterTanks1_wout''"
+                                                      then show "nonPRefsOf (toFr F_CD_3WTsP) v \<noteq> {}"
+                                                      proof (case_tac "v = ''PrWaterTanks2_win''")
+                                                        assume "v = ''PrWaterTanks2_win''"
+                                                        then show "nonPRefsOf (toFr F_CD_3WTsP) v \<noteq> {}"
+                                                        by (simp add: h_NsP nonPRefsOf_def refsOf_def refs_F_CD_3WTsP 
+                                                          trancl_in)
+                                                      next
+                                                        assume h24: "v \<noteq> ''PrWaterTanks2_win''"
+                                                        then show "nonPRefsOf (toFr F_CD_3WTsP) v \<noteq> {}"
+                                                        proof (case_tac "v = ''PrWaterTanks2_wlout''")
+                                                          assume "v = ''PrWaterTanks2_wlout''"
+                                                          then show "nonPRefsOf (toFr F_CD_3WTsP) v \<noteq> {}"
+                                                          by (simp add: h_NsP nonPRefsOf_def refsOf_def refs_F_CD_3WTsP 
+                                                            trancl_in)
+                                                        next
+                                                          assume h25: "v \<noteq> ''PrWaterTanks2_wlout''"
+                                                          then show "nonPRefsOf (toFr F_CD_3WTsP) v \<noteq> {}"
+                                                          proof (case_tac "v = ''PrWaterTanks2_vi''")
+                                                            assume "v = ''PrWaterTanks2_vi''"
+                                                            then show "nonPRefsOf (toFr F_CD_3WTsP) v \<noteq> {}"
+                                                              by (simp add: h_NsP nonPRefsOf_def refsOf_def refs_F_CD_3WTsP 
+                                                                trancl_in)
+                                                          next
+                                                            assume h26: "v \<noteq> ''PrWaterTanks2_vi''"
+                                                            then show "nonPRefsOf (toFr F_CD_3WTsP) v \<noteq> {}"
+                                                            proof (case_tac "v = ''PrTankIOV_vi''")
+                                                              assume "v = ''PrTankIOV_vi''"
+                                                              then show "nonPRefsOf (toFr F_CD_3WTsP) v \<noteq> {}"
+                                                                by (simp add: h_NsP nonPRefsOf_def refsOf_def refs_F_CD_3WTsP 
+                                                                trancl_in)
+                                                            next
+                                                              assume h27: "v \<noteq> ''PrTankIOV_vi''"
+                                                              then show "nonPRefsOf (toFr F_CD_3WTsP) v \<noteq> {}"
+                                                              using h1 h2 h3 h4 h5 h6 h7 h8 h9 h10 h11 h12 h13
+                                                              h14 h15 h16 h17 h18 h19 h20 h21 h22 h23 h24 h25 h26
+                                                              h27 by (simp add: h_NsP)
+                                                            qed
+                                                          qed
+                                                        qed
+                                                      qed
+                                                    qed
+                                                  qed
+                                                qed
+                                              qed
+                                            qed
+                                          qed
+                                        qed
+                                      qed
+                                    qed
+                                  qed
+                                qed
+                              qed
+                            qed
+                          qed
+                        qed
+                      qed
+                    qed
+                  qed
                 qed
               qed
             qed
@@ -936,309 +1353,366 @@ lemma wf_F_CD_3WTs: "is_wf_fr (toFr F_CD_3WTs)"
       qed
     next
       apply_end(rule conjI)
-      have h_wf_g: "is_wf_g (toSGr SG_CD_3WTs)"
-        using wf_SG_CD_3WTs
+      have h_wf_g: "is_wf_g (toSGr SG_CD_3WTsP)"
+        using wf_SG_CD_3WTsP
         by (simp add: is_wf_sg_def)
-      show "acyclic_fr (toFr F_CD_3WTs)"
+      show "acyclic_fr (toFr F_CD_3WTsP)"
       proof -
-          from wf_SG_CD_3WTs have "acyclic (inh (sg (toFr F_CD_3WTs)))"
-            by (simp add: is_wf_sg_def acyclicGr_def inh_def F_CD_3WTs_def toFr_def)
-          then show "acyclic_fr (toFr F_CD_3WTs)"
+          from wf_SG_CD_3WTsP have "acyclic (inh (sg (toFr F_CD_3WTsP)))"
+            by (simp add: is_wf_sg_def acyclicGr_def inh_def F_CD_3WTsP_def toFr_def)
+          then show "acyclic_fr (toFr F_CD_3WTsP)"
           proof (simp add: acyclic_fr_def)
-            assume h1: "acyclic (inh (sg (toFr F_CD_3WTs)))"
-            have h2: "is_wf_g (toSGr (sg_ls (F_CD_3WTs)))"
-              using wf_SG_CD_3WTs by (simp add: F_CD_3WTs_def is_wf_sg_def)
-            have h3: "Domain (inh (sg (toFr F_CD_3WTs))) \<inter> Domain (refs (toFr F_CD_3WTs)) = {}"
+            assume h1: "acyclic (inh (sg (toFr F_CD_3WTsP)))"
+            have h2: "is_wf_g (toSGr (sg_ls (F_CD_3WTsP)))"
+              using wf_SG_CD_3WTsP by (simp add: F_CD_3WTsP_def is_wf_sg_def)
+            have h3: "Domain (inh (sg (toFr F_CD_3WTsP))) \<inter> Domain (refs (toFr F_CD_3WTsP)) = {}"
               using h2 
-                by (simp add: refs_F_CD_3WTs)(simp add: toFr_def inh_eq_consInh, eval)
-            have h4: "Range (refs (toFr F_CD_3WTs)) \<inter> Domain (inh (sg (toFr F_CD_3WTs))) = {}"
-              using h2 by (simp add: refs_F_CD_3WTs)(simp add: toFr_def inh_eq_consInh, eval)
-            have h5: "acyclic(refs (toFr F_CD_3WTs))"
-              by (simp add: refs_F_CD_3WTs)(auto simp add: rtrancl_in acyclic_def)
-            from h1 h3 h4 h5 show "acyclic (inh (sg (toFr F_CD_3WTs)) \<union> refs (toFr F_CD_3WTs))"
+                by (simp add: refs_F_CD_3WTsP)(simp add: toFr_def inh_eq_consInh, eval)
+            have h4: "Range (refs (toFr F_CD_3WTsP)) \<inter> Domain (inh (sg (toFr F_CD_3WTsP))) = {}"
+              using h2 by (simp add: refs_F_CD_3WTsP)(simp add: toFr_def inh_eq_consInh, eval)
+            have h5: "acyclic(refs (toFr F_CD_3WTsP))"
+              by (simp add: refs_F_CD_3WTsP)(auto simp add: rtrancl_in acyclic_def)
+            from h1 h3 h4 h5 show "acyclic (inh (sg (toFr F_CD_3WTsP)) \<union> refs (toFr F_CD_3WTsP))"
               by (simp add: acyclic_Un)
           qed
         qed
     next
-      show "proxies_dont_inherit (toFr F_CD_3WTs)"
+      show "proxies_dont_inherit (toFr F_CD_3WTsP)"
       proof (simp add: proxies_dont_inherit_def, rule equalityI, rule subsetI)
         fix x
-        assume "x \<in> ran (src (sg (toFr F_CD_3WTs)) |` EsI (sg (toFr F_CD_3WTs))) \<inter>
-             NsP (sg (toFr F_CD_3WTs))"
+        assume "x \<in> ran (src (sg (toFr F_CD_3WTsP)) |` EsI (sg (toFr F_CD_3WTsP))) \<inter>
+             NsP (sg (toFr F_CD_3WTsP))"
         then show "x \<in> {}"
         by (simp add: h_NsP)(auto simp add: restrict_map_def 
-          F_CD_3WTs_def toFr_def vimage_def SG_CD_3WTs_def toSGr_def EsI_def EsTy_def ran_def
+          F_CD_3WTsP_def toFr_def vimage_def SG_CD_3WTsP_def toSGr_def EsI_def EsTy_def ran_def
           split: if_splits)
       next
-        show "{} \<subseteq> ran (src (sg (toFr F_CD_3WTs)) |` EsI (sg (toFr F_CD_3WTs))) \<inter> NsP (sg (toFr F_CD_3WTs))"
+        show "{} \<subseteq> ran (src (sg (toFr F_CD_3WTsP)) |` EsI (sg (toFr F_CD_3WTsP))) \<inter> NsP (sg (toFr F_CD_3WTsP))"
         by (simp)
       qed
     qed
   qed
 
-definition T_F_ASD_3WTs :: "MorphL"
+definition T_F_ASD_3WTsP :: "MorphL"
 where
-   "T_F_ASD_3WTs \<equiv> \<lparr>fVL = [(''WaterTanksASD'', ''ASD''), 
-   (''WaterTanksSys'', ''System''), 
-   (''CompWaterTanksSys1'', ''Composition''),
-   (''CompWaterTanksSys2'', ''Composition''), 
-   (''CompWaterTanksSys3'', ''Composition''),
-   (''TanksControl1'', ''EComponent''), 
-   (''TanksControl2'', ''EComponent''),
-   (''CompTanksControl1Valve'', ''Composition''),
-   (''CompTanksControl1WaterTank'', ''Composition''),
-   (''CompTanksControl2WaterTank'', ''Composition''),
-   (''Controller'', ''EComponent''),
-   (''Valve'', ''POComponent''), 
-   (''WaterTank'', ''POComponent''),
-   (''FlowRate'', ''DType''), (''Area'', ''DType''), 
-   (''Height'', ''DType''), (''OpenClosed'', ''Enumeration''),
-   (''WaterTank_win'', ''FlowPort''), (''WaterTank_wout'', ''FlowPort''), 
-   (''Valve_v2'', ''FlowPort''), (''Valve_w'', ''FlowPort''), 
-   (''Controller_v1'', ''FlowPort'')], 
+   "T_F_ASD_3WTsP \<equiv> \<lparr>fVL = [(''3WaterTanksASD'', ''ASD''), 
+    (''3WaterTanksSys'', ''System''), 
+    (''CompWaterTanksSys1'', ''Composition''),
+    (''CompWaterTanksSys2'', ''Composition''), 
+    (''CompWaterTanksSys3'', ''Composition''),
+    (''WaterTanks1'', ''EComponent''), 
+    (''WaterTanks2'', ''EComponent''),  
+    (''Controller'', ''EComponent''), 
+    (''CompWaterTanks1Inflow'', ''Composition''),
+    (''CompWaterTanks1Pipe'', ''Composition''),
+    (''CompWaterTanks1TankIO'', ''Composition''),
+    (''CompWaterTanks2TankIOV'', ''Composition''),
+    (''CompWaterTanks2Drain'', ''Composition''),
+    (''Inflow'', ''POComponent''), (''Pipe'', ''POComponent''), 
+    (''TankIO'', ''POComponent''), (''TankIOV'', ''POComponent''), 
+    (''Drain'', ''POComponent''), (''FlowRate'', ''DType''), 
+    (''WaterLevel'', ''DType''),  (''ValveState'', ''Enumeration''),
+    (''WaterTanks1_wout'', ''FlowPort''), 
+    (''WaterTanks2_win'', ''FlowPort''),  (''WaterTanks2_wlout'', ''FlowPort''), 
+    (''WaterTanks2_vi'', ''FlowPort''), (''Controller_wlin'', ''FlowPort''), 
+    (''Controller_vo'', ''FlowPort''), (''Inflow_wout'', ''FlowPort''), 
+    (''Pipe_win'', ''FlowPort''), (''Pipe_wout'', ''FlowPort''), 
+    (''TankIO_win'', ''FlowPort''), (''TankIO_wout'', ''FlowPort''), 
+    (''TankIOV_win'', ''FlowPort''), (''TankIOV_wout'', ''FlowPort''), 
+    (''TankIOV_wlout'', ''FlowPort''), (''TankIOV_vi'', ''FlowPort''), 
+    (''Drain_win'', ''FlowPort'')], 
     fEL = [
-      (''EWaterTanksASD_WaterTanksSys'', ''Eblocks''), 
-      (''EWaterTanksASD_TanksControl1'', ''Eblocks''), 
-      (''EWaterTanksASD_TanksControl2'', ''Eblocks''), 
-      (''EWaterTanksASD_Valve'', ''Eblocks''), 
-      (''EWaterTanksASD_WaterTank'', ''Eblocks''), 
-      (''EWaterTanksASD_FlowRate'', ''Etypes''), 
-      (''EWaterTanksASD_Area'', ''Etypes''), 
-      (''EWaterTanksASD_Height'', ''Etypes''), 
-      (''EWaterTanksASD_OpenClosed'', ''Etypes''),
-      (''ECompWaterTanksSys1_src'', ''Esrc''),
-      (''ECompWaterTanksSys2_src'', ''Esrc''),
-      (''ECompWaterTanksSys3_src'', ''Esrc''),
-      (''ECompWaterTanksSys1_tgt'', ''Etgt''),
-      (''ECompWaterTanksSys2_tgt'', ''Etgt''),
-      (''ECompWaterTanksSys3_tgt'', ''Etgt''),
-      (''ECompTanksControl1Valve_src'', ''Esrc''),
-      (''ECompTanksControl1WaterTank_src'', ''Esrc''), 
-      (''ECompTanksControl2WaterTank_src'', ''Esrc''),
-      (''ECompTanksControl1Valve_tgt'', ''Etgt''),
-      (''ECompTanksControl1WaterTank_tgt'', ''Etgt''), 
-      (''ECompTanksControl2WaterTank_tgt'', ''Etgt''),
-      (''E_WaterTank_win'', ''EBlockProps''), 
-      (''E_WaterTank_out'', ''EBlockProps''), 
-      (''E_Valve_v2'', ''EBlockProps''), 
-      (''E_Valve_w'', ''EBlockProps''), 
-      (''E_Controller_v1'', ''EBlockProps''),
-      (''E_Dep_w_v2'', ''EFlowPortDepends''), 
-      (''E_Dep_wout_win'', ''EFlowPortDepends'')]\<rparr>"
+      (''E_3WaterTanksASD_3WaterTanksSys'', ''Eblocks''), 
+      (''E_3WaterTanksASD_WaterTanks1'', ''Eblocks''), 
+      (''E_3WaterTanksASD_WaterTanks2'', ''Eblocks''), 
+      (''E_3WaterTanksASD_Controller'', ''Eblocks''), 
+      (''E_3WaterTanksASD_TankIO'', ''Eblocks''), 
+      (''E_3WaterTanksASD_TankIOV'', ''Eblocks''), 
+      (''E_3WaterTanksASD_Inflow'', ''Eblocks''), 
+      (''E_3WaterTanksASD_Pipe'', ''Eblocks''), 
+      (''E_3WaterTanksASD_Drain'', ''Eblocks''), 
+      (''E_3WaterTanksASD_FlowRate'', ''Etypes''), 
+      (''E_3WaterTanksASD_WaterLevel'', ''Etypes''), 
+      (''E_3WaterTanksASD_ValveState'', ''Etypes''), 
+      (''E_CompWaterTanksSys1_src'', ''Esrc''), 
+      (''E_CompWaterTanksSys1_tgt'',  ''Etgt''), 
+      (''E_CompWaterTanksSys2_src'', ''Esrc''), 
+      (''E_CompWaterTanksSys2_tgt'', ''Etgt''), 
+      (''E_CompWaterTanksSys3_src'', ''Esrc''), 
+      (''E_CompWaterTanksSys3_tgt'', ''Etgt''), 
+      (''E_CompWaterTanks1Inflow_src'', ''Esrc''), 
+      (''E_CompWaterTanks1Inflow_tgt'', ''Etgt''),
+      (''E_CompWaterTanks1Pipe_src'', ''Esrc''), 
+      (''E_CompWaterTanks1Pipe_tgt'', ''Etgt''),
+      (''E_CompWaterTanks1TankIO_src'', ''Esrc''), 
+      (''E_CompWaterTanks1TankIO_tgt'', ''Etgt''),
+      (''E_CompWaterTanks2TankIOV_src'', ''Esrc''), 
+      (''E_CompWaterTanks2TankIOV_tgt'', ''Etgt''),
+      (''E_CompWaterTanks2Drain_src'', ''Esrc''), 
+      (''E_CompWaterTanks2Drain_tgt'', ''Etgt''),
+      (''E_WaterTanks1_wout'', ''EBlockProps''),
+      (''E_WaterTanks2_win'', ''EBlockProps''),
+      (''E_WaterTanks2_wlout'', ''EBlockProps''),
+      (''E_WaterTanks2_vi'', ''EBlockProps''),
+      (''E_Controller_wlin'', ''EBlockProps''),
+      (''E_Controller_vo'', ''EBlockProps''),
+      (''E_Inflow_wout'', ''EBlockProps''),
+      (''E_Pipe_win'', ''EBlockProps''),
+      (''E_Pipe_wout'', ''EBlockProps''),
+      (''E_TankIO_win'', ''EBlockProps''),
+      (''E_TankIO_wout'', ''EBlockProps''),
+      (''E_TankIOV_win'', ''EBlockProps''),
+      (''E_TankIOV_wout'', ''EBlockProps''),
+      (''E_TankIOV_wlout'', ''EBlockProps''),
+      (''E_TankIOV_vi'', ''EBlockProps''),
+      (''E_Drain_win'', ''EBlockProps''),
+      (''E_Dep_Pipe_wout_win'', ''EFlowPortDepends''),
+      (''E_Dep_TankIO_wout_win'', ''EFlowPortDepends''),
+      (''E_Dep_WaterTanks2_wlout_win'', ''EFlowPortDepends''),
+      (''E_Dep_TankIOV_wlout_win'', ''EFlowPortDepends''),
+      (''E_Dep_TankIOV_wout_win'', ''EFlowPortDepends''),
+      (''E_Dep_TankIOV_wlout_win'', ''EFlowPortDepends''),
+      (''E_Dep_TankIOV_wout_vi'', ''EFlowPortDepends''),
+      (''E_Dep_Controller_vo_wlin'', ''EFlowPortDepends'')]\<rparr>"
 
 (*Define the other morphism*)
-definition T_F_CD_3WTs :: "MorphL"
+definition T_F_CD_3WTsP :: "MorphL"
 where
-   "T_F_CD_3WTs \<equiv> \<lparr>fVL = [(''PrWaterTank'', ''PrBlock3''), 
-      (''PrValve'', ''PrBlock3''), 
-      (''PrTanksControl1'', ''PrBlock3''), 
-      (''PrTanksControl2'', ''PrBlock3''), 
-      (''PrController'', ''PrBlock3''), 
-      (''CD_3WTs'', ''ConnectionsDiagram''), 
-      (''WTSys'', ''BlockInstance''), 
-      (''V'', ''BlockInstance''), 
-      (''WT1'', ''BlockInstance''), 
-      (''WT2'', ''BlockInstance''), 
-      (''WT3'', ''BlockInstance''), 
-      (''C'', ''BlockInstance''),
-      (''TC1'', ''BlockInstance''), 
-      (''TC2'', ''BlockInstance''), 
-      (''C_w_win1'', ''Connector''), 
-      (''C_wout1_win2'', ''Connector''), 
-      (''C_wout2_win3'', ''Connector''),
-      (''C_v1_v2'', ''Connector''),
-      (''v1'', ''Port''), (''v2'', ''Port''), 
-      (''w'', ''Port''), (''win1'', ''Port''), 
-      (''wout1'', ''Port''), (''win2'', ''Port''), 
-      (''wout2'', ''Port''),
-      (''win3'', ''Port''), (''wout3'', ''Port''), 
-      (''PrValve_v2'', ''PrFlowPort2''), 
-      (''PrValve_w'', ''PrFlowPort2''), 
-      (''PrWaterTank_win'', ''PrFlowPort2''), 
-      (''PrWaterTank_wout'', ''PrFlowPort2''), 
-      (''PrController_v1'', ''PrFlowPort2'')],
-    fEL = [(''ECD_WTSys'', ''ECDblocks''), (''ECD_V'', ''ECDblocks''), 
-      (''ECD_WT1'', ''ECDblocks''), (''ECD_WT2'', ''ECDblocks''),
-      (''ECD_WT3'', ''ECDblocks''), (''ECD_C'', ''ECDblocks''),
-      (''ECD_TC1'', ''ECDblocks''), (''ECD_TC2'', ''ECDblocks''),
-      (''ECD_C_v1_v2'', ''ECDconnectors''), (''ECD_C_w_win1'', ''ECDconnectors''),
-      (''ECD_C_wout1_win2'', ''ECDconnectors''), 
-      (''ECD_C_wout2_win3'', ''ECDconnectors''),
-      (''E_C_v1_v2_src'', ''EC_src''), (''E_C_v1_v2_tgt'', ''EC_tgt''), 
-      (''E_C_w_win1_src'', ''EC_src''), (''E_C_w_win1_tgt'', ''EC_tgt''), 
-      (''E_C_wout1_win2_src'', ''EC_src''), (''E_C_wout1_win2_tgt'', ''EC_tgt''), 
-      (''E_C_wout2_win3_src'', ''EC_src''), (''E_C_wout2_win3_tgt'', ''EC_tgt''), 
-      (''E_C_v1'', ''EBIports''), (''E_V_v2'', ''EBIports''),   
-      (''E_V_w'', ''EBIports''), 
-      (''E_WT1_win1'', ''EBIports''),
-      (''E_WT1_wout1'', ''EBIports''), 
-      (''E_WT2_win2'', ''EBIports''),
-      (''E_WT2_wout2'', ''EBIports''), 
-      (''E_WT3_win3'', ''EBIports''), 
-      (''E_WT3_wout3'', ''EBIports''), (''E_v1_ty'', ''EPortType''), 
-      (''E_v2_ty'', ''EPortType''), (''E_w_ty'', ''EPortType''),
-      (''E_win1_ty'', ''EPortType''), 
-      (''E_wout1_ty'', ''EPortType''),
-      (''E_win2_ty'', ''EPortType''), (''E_wout2_ty'', ''EPortType''), 
-      (''E_win3_ty'', ''EPortType''), (''E_wout3_ty'', ''EPortType''),
-      (''ERPrWaterTank'', ''ERPrBlock3''), (''ERPrValve'', ''ERPrBlock3''), 
-      (''ERPrTanksControl1'', ''ERPrBlock3''), 
-      (''ERPrTanksControl2'', ''ERPrBlock3''),
-      (''ERPrController'', ''ERPrBlock3''), 
-      (''ERPrValve_v2'', ''ERPrFlowPort2''),
-      (''ERPrValve_w'', ''ERPrFlowPort2''), 
-      (''ERPrWaterTank_win'', ''ERPrFlowPort2''),
-      (''ERPrWaterTank_wout'', ''ERPrFlowPort2''), 
-      (''ERPrController_v1'', ''ERPrFlowPort2'')]\<rparr>"
+   "T_F_CD_3WTsP \<equiv> \<lparr>fVL = [
+    (''PrTankIO'', ''PrBlock3''), (''PrTankIOV'', ''PrBlock3''), 
+    (''PrInflow'', ''PrBlock3''), (''PrPipe'', ''PrBlock3''), 
+    (''PrDrain'', ''PrBlock3''), (''PrWaterTanks1'', ''PrBlock3''), 
+    (''PrWaterTanks2'', ''PrBlock3''), (''PrController'', ''PrBlock3''), 
+    (''CD_3WTs'', ''ConnectionsDiagram''), (''WTSys'', ''BlockInstance''), 
+    (''I'', ''BlockInstance''), (''P'', ''BlockInstance''), (''T1'', ''BlockInstance''), 
+    (''T2'', ''BlockInstance''), (''T3'', ''BlockInstance''),  
+    (''C'', ''BlockInstance''), (''D'', ''BlockInstance''), 
+    (''WT1'', ''BlockInstance''), (''WT2'', ''BlockInstance''),
+    (''iout'', ''Port''), (''t1in'', ''Port''), (''t1out'', ''Port''),
+    (''pin'', ''Port''), (''pout'', ''Port''), (''t2in'', ''Port''),
+    (''t2out'', ''Port''), (''wout'', ''Port''), (''win'', ''Port''),
+    (''wlout'', ''Port''), (''vi1'', ''Port''), (''t3in'', ''Port''),
+    (''t3wlout'', ''Port''), (''t3out'', ''Port''), (''vi2'', ''Port''),
+    (''din'', ''Port''), (''din'', ''Port''), (''wlin'', ''Port''), 
+    (''vo'', ''Port''), 
+    (''C_iout_t1in'', ''Connector''), (''C_t1out_pin'', ''Connector''), 
+    (''C_pout_t2in2'', ''Connector''), (''C_t2out_wout'', ''Connector''), 
+    (''C_wout_win'', ''Connector''),  (''C_win_t3in'', ''Connector''), 
+    (''C_t3wlout_wlout'', ''Connector''), (''C_t3out_din'', ''Connector''), 
+    (''C_wlout_wlin'', ''Connector''), (''C_vo_vi1'', ''Connector''), 
+    (''C_vi1_vi2'', ''Connector''), (''PrInflow_wout'', ''PrFlowPort2''), 
+    (''PrTankIO_win'', ''PrFlowPort2''), (''PrTankIO_wout'', ''PrFlowPort2''), 
+    (''PrPipe_win'', ''PrFlowPort2''), (''PrPipe_wout'', ''PrFlowPort2''), 
+    (''PrWaterTanks1_wout'', ''PrFlowPort2''), (''PrWaterTanks2_win'', ''PrFlowPort2''),
+    (''PrWaterTanks2_wlout'', ''PrFlowPort2''), (''PrWaterTanks2_vi'', ''PrFlowPort2''),
+    (''PrController_wlin'', ''PrFlowPort2''), (''PrController_vo'', ''PrFlowPort2''),
+    (''PrDrain_win'', ''PrFlowPort2''), (''PrTankIOV_win'', ''PrFlowPort2''),
+    (''PrTankIOV_wout'', ''PrFlowPort2''), (''PrTankIOV_wlout'', ''PrFlowPort2''),
+    (''PrTankIOV_vi'', ''PrFlowPort2'')],
+    fEL = [(''ECD_WTSys'', ''ECDblocks''),
+      (''ECD_I'', ''ECDblocks''), (''ECD_P'', ''ECDblocks''),
+      (''ECD_T1'', ''ECDblocks''), (''ECD_T2'',  ''ECDblocks''),
+      (''ECD_T3'', ''ECDblocks''), (''ECD_C'', ''ECDblocks''), 
+      (''ECD_D'', ''ECDblocks''), (''ECD_WT1'', ''ECDblocks''), 
+      (''ECD_WT2'', ''ECDblocks''), (''ECD_C_iout_t1in'', ''ECDconnectors''),
+      (''ECD_C_t1out_pin'', ''ECDconnectors''), (''ECD_C_pout_t2in2'', ''ECDconnectors''),
+      (''ECD_C_t2out_wout'', ''ECDconnectors''), (''ECD_C_wout_win'', ''ECDconnectors''),
+      (''ECD_C_win_t3in'', ''ECDconnectors''), (''ECD_C_t3wlout_wlout'', ''ECDconnectors''),
+      (''ECD_C_t3out_din'', ''ECDconnectors''), (''ECD_C_wlout_wlin'', ''ECDconnectors''),
+      (''ECD_C_vo_vi1'', ''ECDconnectors''), (''ECD_C_vi1_vi2'', ''ECDconnectors''),
+      (''E_WTSys_WT1'', ''EBIInside''), (''E_WTSys_WT2'', ''EBIInside''),
+      (''E_WTSys_C'', ''EBIInside''), (''E_WT1_I'', ''EBIInside''),
+      (''E_WT1_P'', ''EBIInside''), (''E_WT1_T1'', ''EBIInside''), 
+      (''E_WT1_T2'', ''EBIInside''), (''E_WT2_T3'', ''EBIInside''),
+      (''E_WT2_D'', ''EBIInside''), (''E_I_iout'', ''EBIports''), 
+      (''E_P_pin'', ''EBIports''), (''E_P_pout'', ''EBIports''), 
+      (''E_T1_t1in'', ''EBIports''), (''E_T1_t1out'', ''EBIports''),
+      (''E_T2_t2in'', ''EBIports''), (''E_T2_t2out'', ''EBIports''),
+      (''E_T3_t3in'', ''EBIports''), (''E_T3_t3wlout'', ''EBIports''),
+      (''E_T3_vi2'', ''EBIports''), (''E_C_wlin'', ''EBIports''),
+      (''E_C_vo'', ''EBIports''), (''E_D_din'', ''EBIports''),
+      (''E_WT1_wout'', ''EBIports''), (''E_WT2_win'', ''EBIports''),
+      (''E_WT2_wlout'', ''EBIports''), (''E_WT2_vi1'', ''EBIports''),
+      (''E_C_iout_t1in_src'', ''EC_src''), (''E_C_iout_t1in_tgt'', ''EC_tgt''),
+      (''E_C_t1out_pin_src'', ''EC_src''), (''E_C_t1out_pin_tgt'', ''EC_tgt''),
+      (''E_C_pout_t2in_src'', ''EC_src''), (''E_C_pout_t2in_tgt'', ''EC_tgt''),
+      (''E_C_t2out_wout_src'', ''EC_src''), (''E_C_t2out_wout_tgt'', ''EC_tgt''),
+      (''E_C_wout_win_src'', ''EC_src''), (''E_C_wout_win_tgt'', ''EC_tgt''),
+      (''E_C_win_t3in_src'', ''EC_src''), (''E_C_win_t3in_tgt'', ''EC_tgt''),
+      (''E_C_t3wlout_wlout_src'', ''EC_src''), (''E_C_t3wlout_wlout_tgt'', ''EC_tgt''),
+      (''E_C_t3out_din_src'', ''EC_src''), (''E_C_t3out_din_tgt'', ''EC_tgt''),
+      (''E_C_wlout_wlin_src'', ''EC_src''), (''E_C_wlout_wlin_tgt'', ''EC_tgt''),
+      (''E_C_vo_vi1_src'', ''EC_src''),  (''E_C_vo_vi1_tgt'', ''EC_tgt''),
+      (''E_C_vi1_vi2_src'', ''EC_src''), (''E_C_vi1_vi2_tgt'', ''EC_tgt''),
+      (''E_iout_ty'', ''EPortType''), (''E_t1in_ty'', ''EPortType''), 
+      (''E_t1out_ty'', ''EPortType''), (''E_pin_ty'', ''EPortType''), 
+      (''E_pout_ty'', ''EPortType''), (''E_t2in_ty'', ''EPortType''),
+      (''E_t2out_ty'', ''EPortType''), (''E_wout_ty'', ''EPortType''), 
+      (''E_win_ty'', ''EPortType''), (''E_wlout_ty'', ''EPortType''),
+      (''E_vi1_ty'', ''EPortType''), (''E_t3in_ty'', ''EPortType''),
+      (''E_t3wlout_ty'', ''EPortType''), (''E_t3out_ty'', ''EPortType''), 
+      (''E_vi2_ty'', ''EPortType''), (''E_din_ty'', ''EPortType''), 
+      (''E_wlin_ty'', ''EPortType''), (''E_vo_ty'', ''EPortType''),
+      (''ERPrTankIO'', ''ERPrBlock3''), (''ERPrTankIOV'', ''ERPrBlock3''), 
+      (''ERPrInflow'', ''ERPrBlock3''), (''ERPrPipe'', ''ERPrBlock3''),
+      (''ERPrDrain'', ''ERPrBlock3''), (''ERPrWaterTanks1'', ''ERPrBlock3''),
+      (''ERPrWaterTanks2'', ''ERPrBlock3''), (''ERPrController'', ''ERPrBlock3''),
+      (''ERPrInflow_wout'', ''ERPrBlock3''), (''ERPrTankIO_win'', ''ERPrBlock3''),
+      (''ERPrTankIO_wout'', ''ERPrBlock3''), (''ERPrPipe_win'', ''ERPrBlock3''),
+      (''ERPrPipe_wout'', ''ERPrBlock3''), (''ERPrWaterTanks1_wout'', ''ERPrBlock3''),
+      (''ERPrWaterTanks2_win'', ''ERPrBlock3''), (''ERPrWaterTanks2_wlout'', ''ERPrBlock3''),
+      (''ERPrWaterTanks2_vi'', ''ERPrBlock3''),(''ERPrController_wlin'', ''ERPrBlock3''),
+      (''ERPrController_vo'', ''ERPrBlock3''), (''ERPrDrain_win'', ''ERPrBlock3''),
+      (''ERPrTankIOV_win'', ''ERPrBlock3''), (''ERPrTankIOV_wout'', ''ERPrBlock3''),
+      (''ERPrTankIOV_wlout'', ''ERPrBlock3''), (''ERPrTankIOV_vi'', ''ERPrBlock3'')]\<rparr>"
 
-definition GFG_3WTs :: "GFGr_ls"
+definition GFG_3WTsP :: "GFGr_ls"
 where
-  "GFG_3WTs \<equiv> 
-    \<lparr>NsG = [''F_ASD_3WTs'', ''F_CD_3WTs''], 
-      EsG= [''E_F_CD_3WTs_ASD'', ''E_F_ASD_3WTs'', ''E_F_CD_3WTs''], 
-      srcG = [(''E_F_CD_3WTs_ASD'', ''F_CD_3WTs''), 
-        (''E_F_ASD_3WTs'', ''F_ASD_3WTs''),
-        (''E_F_CD_3WTs'', ''F_CD_3WTs'')],
-      tgtG = [(''E_F_CD_3WTs_ASD'', ''F_ASD_3WTs''), 
-        (''E_F_ASD_3WTs'', ''F_ASD_3WTs''),
-        (''E_F_CD_3WTs'', ''F_CD_3WTs'')],
-      ext_ty_ls = [(''E_F_CD_3WTs_ASD'', eimp), (''E_F_ASD_3WTs'', eimp),
-        (''E_F_CD_3WTs'', eimp)]\<rparr>"
+  "GFG_3WTsP \<equiv> 
+    \<lparr>NsG = [''F_ASD_3WTsP'', ''F_CD_3WTsP''], 
+      EsG= [''E_F_CD_3WTsP_ASD'', ''E_F_ASD_3WTsP'', ''E_F_CD_3WTsP''], 
+      srcG = [(''E_F_CD_3WTsP_ASD'', ''F_CD_3WTsP''), 
+        (''E_F_ASD_3WTsP'', ''F_ASD_3WTsP''),
+        (''E_F_CD_3WTsP'', ''F_CD_3WTsP'')],
+      tgtG = [(''E_F_CD_3WTsP_ASD'', ''F_ASD_3WTsP''), 
+        (''E_F_ASD_3WTsP'', ''F_ASD_3WTsP''),
+        (''E_F_CD_3WTsP'', ''F_CD_3WTsP'')],
+      ext_ty_ls = [(''E_F_CD_3WTsP_ASD'', eimp), (''E_F_ASD_3WTsP'', eimp),
+        (''E_F_CD_3WTsP'', eimp)]\<rparr>"
 
 axiomatization
 where
-  Es_GFG_3WTs: "Es (toGFGr(GFG_3WTs)) \<subseteq> E_A"
-  and Ns_GFG_3WTs: "Ns (toGFGr(GFG_3WTs)) \<subseteq> V_A"
+  Es_GFG_3WTsP: "Es (toGFGr(GFG_3WTsP)) \<subseteq> E_A"
+  and Ns_GFG_3WTsP: "Ns (toGFGr(GFG_3WTsP)) \<subseteq> V_A"
 
-lemma is_wf_GFG_3WTs: "is_wf_gfg_ls GFG_3WTs"
+lemma is_wf_GFG_3WTs: "is_wf_gfg_ls GFG_3WTsP"
   proof -
-    have h_wf_g: "is_wf_g (toGFGr GFG_3WTs)"
-      using Es_GFG_3WTs Ns_GFG_3WTs
-        by (auto simp add: is_wf_g_def GFG_3WTs_def ftotal_on_def toGFGr_def)
+    have h_wf_g: "is_wf_g (toGFGr GFG_3WTsP)"
+      using Es_GFG_3WTsP Ns_GFG_3WTsP
+        by (simp add: is_wf_g_def GFG_3WTsP_def ftotal_on_def toGFGr_def)
     show ?thesis
     proof (simp add: is_wf_gfg_ls_def, rule conjI)
-      show "distinct (NsG GFG_3WTs)"
-      by (simp add: GFG_3WTs_def)
+      show "distinct (NsG GFG_3WTsP)"
+      by (simp add: GFG_3WTsP_def)
     next
       apply_end(rule conjI)
-      show "distinct (map fst (srcG GFG_3WTs))"
-        by (simp add: GFG_3WTs_def)
+      show "distinct (map fst (srcG GFG_3WTsP))"
+        by (simp add: GFG_3WTsP_def)
     next
       apply_end(rule conjI)
-      show "distinct (map fst (tgtG GFG_3WTs))"
-        by (simp add: GFG_3WTs_def)
+      show "distinct (map fst (tgtG GFG_3WTsP))"
+        by (simp add: GFG_3WTsP_def)
     next
-      show "is_wf_gfg (toGFGr GFG_3WTs)"
+      show "is_wf_gfg (toGFGr GFG_3WTsP)"
         proof (simp add: is_wf_gfg_def, rule conjI)
-          show "is_wf_g (toGFGr GFG_3WTs)"
+          show "is_wf_g (toGFGr GFG_3WTsP)"
             using h_wf_g by simp
         next
           apply_end (rule conjI)
-          show "ftotal_on (ext_ty (toGFGr GFG_3WTs)) (Es (toGFGr GFG_3WTs)) GFGEdgeTy_set"
-            by (simp add: GFG_3WTs_def toGFGr_def GFGEdgeTy_set_def ftotal_on_def)
+          show "ftotal_on (ext_ty (toGFGr GFG_3WTsP)) (Es (toGFGr GFG_3WTsP)) GFGEdgeTy_set"
+            by (simp add: GFG_3WTsP_def toGFGr_def GFGEdgeTy_set_def ftotal_on_def)
         next
           apply_end (rule conjI)
-          show "NodesWithSelfEdges (toGFGr GFG_3WTs)"
+          show "NodesWithSelfEdges (toGFGr GFG_3WTsP)"
           proof (simp add: NodesWithSelfEdges_def, clarify)
             fix v
-            assume "v \<in> Ns (toGFGr GFG_3WTs)"
-            then have h1: "v = ''F_CD_3WTs'' \<or> v = ''F_ASD_3WTs''"
-              by (auto simp add: GFG_3WTs_def toGFGr_def)
-            then show "\<exists>e. e \<in> Es (toGFGr GFG_3WTs) 
-              \<and> src (toGFGr GFG_3WTs) e = Some v 
-              \<and> tgt (toGFGr GFG_3WTs) e = Some v"
-            by (simp add:  GFG_3WTs_def toGFGr_def NodesWithSelfEdges_def)
-              (erule disjE, rule exI[where x= "''E_F_CD_3WTs''"], simp_all, 
-                rule exI[where x= "''E_F_ASD_3WTs''"], simp)
+            assume "v \<in> Ns (toGFGr GFG_3WTsP)"
+            then have h1: "v = ''F_CD_3WTsP'' \<or> v = ''F_ASD_3WTsP''"
+              by (auto simp add: GFG_3WTsP_def toGFGr_def)
+            then show "\<exists>e. e \<in> Es (toGFGr GFG_3WTsP) 
+              \<and> src (toGFGr GFG_3WTsP) e = Some v 
+              \<and> tgt (toGFGr GFG_3WTsP) e = Some v"
+            by (simp add:  GFG_3WTsP_def toGFGr_def NodesWithSelfEdges_def)
+              (erule disjE, simp, rule exI[where x="''E_F_ASD_3WTsP''"], simp)
           qed
         next
           show "acyclicGr
-            (restrict (toGFGr GFG_3WTs)
-              (Es (toGFGr GFG_3WTs) - EsId (toGFGr GFG_3WTs)))"
-          by (auto simp add: GFG_3WTs_def toGFGr_def EsId_def restrict_def acyclicGr_def
+            (restrict (toGFGr GFG_3WTsP)
+              (Es (toGFGr GFG_3WTsP) - EsId (toGFGr GFG_3WTsP)))"
+          by (auto simp add: GFG_3WTsP_def toGFGr_def EsId_def restrict_def acyclicGr_def
             relOfGr_def rst_Ns_def rst_fun_def adjacent_def acyclic_def elim: tranclE)
      qed
    qed
   qed
 
-definition Mdl_3WTs :: "Mdl_ls"
+definition Mdl_3WTsP :: "Mdl_ls"
 where
-  "Mdl_3WTs \<equiv> \<lparr>gfgL = GFG_3WTs, 
-    frdL = [(''F_ASD_3WTs'', F_ASD_3WTs), (''F_CD_3WTs'', F_CD_3WTs)]\<rparr>"
+  "Mdl_3WTsP \<equiv> \<lparr>gfgL = GFG_3WTsP, 
+    frdL = [(''F_ASD_3WTsP'', F_ASD_3WTsP), (''F_CD_3WTsP'', F_CD_3WTsP)]\<rparr>"
 
-lemma is_wf_mdl_3WTs: "is_wf_mdl (toMdl Mdl_3WTs)"
+lemma is_wf_mdl_3WTs: "is_wf_mdl (toMdl Mdl_3WTsP)"
   proof (simp add: is_wf_mdl_def, rule conjI)
-    show "\<forall>F. F \<in> ran (frd (toMdl Mdl_3WTs)) \<longrightarrow> is_wf_fr F"
+    show "\<forall>F. F \<in> ran (frd (toMdl Mdl_3WTsP)) \<longrightarrow> is_wf_fr F"
     proof (clarify)
       fix F
-      assume "F \<in> ran (frd (toMdl Mdl_3WTs))"
-      then have h1: "F = (toFr F_ASD_3WTs) \<or> F = (toFr F_CD_3WTs)"
-        by (auto simp add: INTO_SysML_MM_def toMdl_def Mdl_3WTs_def)
+      assume "F \<in> ran (frd (toMdl Mdl_3WTsP))"
+      then have h1: "F = (toFr F_ASD_3WTsP) \<or> F = (toFr F_CD_3WTsP)"
+        by (auto simp add: INTO_SysML_MM_def toMdl_def Mdl_3WTsP_def)
       then show "is_wf_fr F"
-      proof (case_tac "F = toFr F_ASD_3WTs")
-        assume "F = toFr F_ASD_3WTs"
+      proof (case_tac "F = toFr F_ASD_3WTsP")
+        assume "F = toFr F_ASD_3WTsP"
         then show "is_wf_fr F"
-          by (simp add: wf_F_ASD_3WTs)
+          by (simp add: wf_F_ASD_3WTsP)
       next
-        assume h2: "F \<noteq> toFr F_ASD_3WTs"
+        assume h2: "F \<noteq> toFr F_ASD_3WTsP"
         then show "is_wf_fr F"
-        proof (case_tac "F = toFr F_CD_3WTs")
-          assume "F = toFr F_CD_3WTs"
+        proof (case_tac "F = toFr F_CD_3WTsP")
+          assume "F = toFr F_CD_3WTsP"
           then show "is_wf_fr F"
             by (simp add: wf_F_CD_3WTs)
         next
-          assume h3: "F \<noteq> toFr F_CD_3WTs"
+          assume h3: "F \<noteq> toFr F_CD_3WTsP"
           then show "is_wf_fr F" using h1 h2 by (simp)
         qed
       qed
     qed
   next
     apply_end(rule conjI)
-    show "is_wf_gfg_ls (gfg (toMdl Mdl_3WTs))"
-      by (simp add: is_wf_GFG_3WTs Mdl_3WTs_def toMdl_def)
+    show "is_wf_gfg_ls (gfg (toMdl Mdl_3WTsP))"
+      by (simp add: is_wf_GFG_3WTs Mdl_3WTsP_def toMdl_def)
   next
     apply_end(rule conjI)
-    show "ftotal_on (frd (toMdl Mdl_3WTs)) (set (NsG (gfg (toMdl Mdl_3WTs)))) fr_set"
-      by (simp add: ftotal_on_def Mdl_3WTs_def toMdl_def GFG_3WTs_def F_ASD_3WTs_def
-        toFr_def toSGr_def SG_ASD_3WTs_def F_CD_3WTs_def fr_set_def is_fr_def)
+    show "ftotal_on (frd (toMdl Mdl_3WTsP)) (set (NsG (gfg (toMdl Mdl_3WTsP)))) fr_set"
+      by (simp add: ftotal_on_def Mdl_3WTsP_def toMdl_def GFG_3WTsP_def F_ASD_3WTsP_def
+        toFr_def toSGr_def SG_ASD_3WTsP_def F_CD_3WTsP_def fr_set_def is_fr_def)
   next
     apply_end(rule conjI)
-    show "disjMdlFrs (toMdl Mdl_3WTs)"
-      by (simp add: disjMdlFrs_def Mdl_3WTs_def disjFs_def disjGsL_def 
-        GFG_3WTs_def F_Common_def SG_F_Common_def F_Props_def SG_F_Props_def
-        toFr_def toMdl_def toSGr_def SG_ASD_3WTs_def SG_CD_3WTs_def
-        F_ASD_3WTs_def F_CD_3WTs_def)
+    show "disjMdlFrs (toMdl Mdl_3WTsP)"
+      by (simp add: disjMdlFrs_def Mdl_3WTsP_def disjFs_def disjGsL_def 
+        GFG_3WTsP_def F_Common_def SG_F_Common_def F_Props_def SG_F_Props_def
+        toFr_def toMdl_def toSGr_def SG_ASD_3WTsP_def SG_CD_3WTsP_def
+        F_ASD_3WTsP_def F_CD_3WTsP_def)
   next
-    show "mUM2GFG (toMdl Mdl_3WTs)
-      \<in> morphF2GFGr (UMdlFs (toMdl Mdl_3WTs)) (toGFGr (gfg (toMdl Mdl_3WTs)))"
+    show "mUM2GFG (toMdl Mdl_3WTsP)
+      \<in> morphF2GFGr (UMdlFs (toMdl Mdl_3WTsP)) (toGFGr (gfg (toMdl Mdl_3WTsP)))"
       by (simp add: UGM_eq_ConsUGM)
   qed
 
-definition MdlTy_3WTs :: "MdlTy_ls"
+definition MdlTy_3WTsP :: "MdlTy_ls"
 where
-  "MdlTy_3WTs \<equiv> \<lparr>tmdlL = INTO_SysML_MM_T, 
-    mdlL = Mdl_3WTs,
-    mtyL = (consUGM T_F_ASD_3WTs T_F_CD_3WTs)\<rparr>"
+  "MdlTy_3WTsP \<equiv> \<lparr>tmdlL = INTO_SysML_MM_T, 
+    mdlL = Mdl_3WTsP,
+    mtyL = (consUGM T_F_ASD_3WTsP T_F_CD_3WTsP)\<rparr>"
 
-lemma is_wf_mdlt_3WTs: "is_wf_mdlty (toMdlTy MdlTy_3WTs)"
+lemma is_wf_mdlt_3WTsP: "is_wf_mdlty (toMdlTy MdlTy_3WTsP)"
   proof (simp add: is_wf_mdlty_def, rule conjI)
-    show "is_wf_tmdl (tmdl (toMdlTy MdlTy_3WTs))"
-      by (simp add: is_wf_INTO_SysML_MM_T MdlTy_3WTs_def toMdlTy_def)
+    show "is_wf_tmdl (tmdl (toMdlTy MdlTy_3WTsP))"
+      by (simp add: is_wf_INTO_SysML_MM_T MdlTy_3WTsP_def toMdlTy_def)
   next
     apply_end(rule conjI)
-    show "is_wf_mdl (mdl (toMdlTy MdlTy_3WTs))"
-      by (simp add: is_wf_mdl_3WTs toMdlTy_def MdlTy_3WTs_def)
+    show "is_wf_mdl (mdl (toMdlTy MdlTy_3WTsP))"
+      by (simp add: is_wf_mdl_3WTs toMdlTy_def MdlTy_3WTsP_def)
   next
-    show "mty (toMdlTy MdlTy_3WTs)
-    \<in> morphFr (UMdlFs (mdl (toMdlTy MdlTy_3WTs))) (fr (UTyMdlFs (tmdl (toMdlTy MdlTy_3WTs))))"
-    by (simp add: toMdlTy_def MdlTy_3WTs_def)
+    show "mty (toMdlTy MdlTy_3WTsP)
+    \<in> morphFr (UMdlFs (mdl (toMdlTy MdlTy_3WTsP))) (fr (UTyMdlFs (tmdl (toMdlTy MdlTy_3WTsP))))"
+    by (simp add: toMdlTy_def MdlTy_3WTsP_def)
   qed
 
-value "consUMdlFs (mdlL MdlTy_3WTs)"
+value "consUMdlFs (mdlL MdlTy_3WTsP)"
  
-value "INTO_SysML_toPDG_Nodes (mdlL MdlTy_3WTs) (toMorph (mtyL MdlTy_3WTs))"
+value "INTO_SysML_toPDG_Nodes (mdlL MdlTy_3WTsP) (toMorph (mtyL MdlTy_3WTsP))"
 
-value "INTO_SysML_toPDG (mdlL MdlTy_3WTs) (toMorph (mtyL MdlTy_3WTs))"
+value "INTO_SysML_toPDG MdlTy_3WTsP"
 
 fun portNodes :: "Mdl_ls \<Rightarrow> Morph \<Rightarrow> V list"
 where
@@ -1250,35 +1724,24 @@ where
    "edgesOfTy ML m e = 
     (filter (\<lambda>v . (fE m) v = Some e )((EsG o sg_ls) (consUMdlFs ML)))"
 
-value "portNodes (mdlL MdlTy_3WTs) (toMorph (mtyL MdlTy_3WTs))"
+value "portNodes (mdlL MdlTy_3WTsP) (toMorph (mtyL MdlTy_3WTsP))"
 
-value "edgesOfTy (mdlL MdlTy_3WTs) (toMorph (mtyL MdlTy_3WTs)) ''EPortType''"
+value "edgesOfTy (mdlL MdlTy_3WTsP) (toMorph (mtyL MdlTy_3WTsP)) ''EPortType''"
 
-value "edgesOfTy (mdlL MdlTy_3WTs) (toMorph (mtyL MdlTy_3WTs)) ''EFlowPortDepends''"
+value "edgesOfTy (mdlL MdlTy_3WTsP) (toMorph (mtyL MdlTy_3WTsP)) ''EFlowPortDepends''"
 
-value "edgesOfTy (mdlL MdlTy_3WTs) (toMorph (mtyL MdlTy_3WTs)) ''EBIports''"
-
-value "the (tgt (sg (toFr (consUMdlFs (mdlL MdlTy_3WTs)))) ''E_WT3_win3'')"
-
-value "the (tgt (sg (toFr (consUMdlFs (mdlL MdlTy_3WTs)))) ''E_v2_ty'')"
-
-value "(set (consSrcStF (consUMdlFs (mdlL MdlTy_3WTs)))) ``{''E_Dep_w_v2''}"
-
-value "the (tgt (sg (toFr (consUMdlFs (mdlL MdlTy_3WTs)))) ''E_Dep_w_v2'')"
+value "edgesOfTy (mdlL MdlTy_3WTsP) (toMorph (mtyL MdlTy_3WTsP)) ''EBIports''"
 
 (*Get these functions right*)
-value "getBlockInstanceOfPort (toMorph (mtyL MdlTy_3WTs)) (consUMdlFs (mdlL MdlTy_3WTs)) ''win3''"
-value "getOtherInternalPorts (toMorph (mtyL MdlTy_3WTs)) (consUMdlFs (mdlL MdlTy_3WTs)) ''win3''"
-value "getFlowPortTypeOfPort (toMorph (mtyL MdlTy_3WTs)) (consUMdlFs (mdlL MdlTy_3WTs)) ''win3''"
+value "getBlockInstanceOfPort (toMorph (mtyL MdlTy_3WTsP)) (consUMdlFs (mdlL MdlTy_3WTsP)) ''t1in''"
+value "getOtherInternalPorts (toMorph (mtyL MdlTy_3WTsP)) (consUMdlFs (mdlL MdlTy_3WTsP)) ''t1in''"
+value "getFlowPortTypeOfPort (toMorph (mtyL MdlTy_3WTsP)) (consUMdlFs (mdlL MdlTy_3WTsP)) ''iout''"
 
 (*
 value "getDependentPortOfV (mty_ls MdlTy_3WTs) (consUMdlFs (mdl_ls MdlTy_3WTs)) ''w'' ''PrValve_v2''"
 *)
-value "(fV (toMorph (mtyL MdlTy_3WTs))) (the (tgt (sg (toFr (consUMdlFs (mdlL MdlTy_3WTs)))) ''E_v2_ty''))"
 
-value "(set(consTgtStF (consUMdlFs (mdlL MdlTy_3WTs)))) ``{''E_v2_ty''}"
-
-value "consClanF ''PrController_v1'' (consUMdlFs (mdlL MdlTy_3WTs))"
+value "consClanF ''PrController_vo'' (consUMdlFs (mdlL MdlTy_3WTsP))"
 
 fun internalConnectionsOf :: "Mdl_ls \<Rightarrow> Morph \<Rightarrow> V \<Rightarrow> Gr_ls"
 where
@@ -1291,8 +1754,8 @@ where
     (filter (\<lambda> e. (getFlowPortTypeOfPort m (consUMdlFs ML) v) \<in> (set (consSrcStF (consUMdlFs ML))) ``{e})
             (filter (\<lambda> e. (fE m) e = Some ''EFlowPortDepends'') (EsG (sg_ls (consUMdlFs ML)))))"
 
-value "buildGrForConnector (toMorph (mtyL MdlTy_3WTs)) (consUMdlFs (mdlL MdlTy_3WTs)) ''C_w_win1''"
-value "dependsGrOf (mdlL MdlTy_3WTs) (toMorph (mtyL MdlTy_3WTs)) ''win3''"
-value "internalConnectionsOf (mdlL MdlTy_3WTs) (toMorph (mtyL MdlTy_3WTs)) ''w''"
+value "buildGrForConnector (toMorph (mtyL MdlTy_3WTsP)) (consUMdlFs (mdlL MdlTy_3WTsP)) ''C_wout_win''"
+value "dependsGrOf (mdlL MdlTy_3WTsP) (toMorph (mtyL MdlTy_3WTsP)) ''iout''"
+value "internalConnectionsOf (mdlL MdlTy_3WTsP) (toMorph (mtyL MdlTy_3WTsP)) ''iout''"
 
 end
